ems/SimModSem.v
@@ -20,22 +20,13 @@ Set Implicit Arguments.
 
 Local Open Scope nat_scope.
 
-
-
-
-
-
-
-
-
-
 Section SIM.
   Let st_local: Type := (Any.t).
 
   Variable world: Type.
 
   Let W: Type := (Any.t) * (Any.t).
-  Variable wf: world -> W -> Prop.
+  Variable wf : world -> W -> Prop.
   Variable le: relation world.
 
 
@@ -47,16 +38,18 @@ Section SIM.
       v_src v_tgt
       (RET: RR st_src0 st_tgt0 v_src v_tgt)
     :
-      _sim_itree sim_itree RR i_src0 i_tgt0 w0 (st_src0, (Ret v_src)) (st_tgt0, (Ret v_tgt))
+      _sim_itree sim_itree RR i_src0 i_tgt0 w0 (st_src0, Ret v_src) (st_tgt0, Ret v_tgt)
+
   | sim_itree_call
       i_src0 i_tgt0 w w0 st_src0 st_tgt0
       fn varg k_src k_tgt
       (WF: wf w0 (st_src0, st_tgt0))
       (K: forall w1 vret st_src1 st_tgt1 (WLE: le w0 w1) (WF: wf w1 (st_src1, st_tgt1)),
-          sim_itree _ _ RR true true w (st_src1, k_src vret) (st_tgt1, k_tgt vret))
+          sim_itree _ _ RR false false w (st_src1, k_src vret) (st_tgt1, k_tgt vret))
     :
       _sim_itree sim_itree RR i_src0 i_tgt0 w (st_src0, trigger (Call fn varg) >>= k_src)
                  (st_tgt0, trigger (Call fn varg) >>= k_tgt)
+
   | sim_itree_syscall
       i_src0 i_tgt0 w0 st_src0 st_tgt0
       fn varg rvs k_src k_tgt
@@ -67,84 +60,69 @@ Section SIM.
                  (st_tgt0, trigger (Syscall fn varg rvs) >>= k_tgt)
 
   | sim_itree_tau_src
-      i_src0 i_tgt0 w0 st_src0 st_tgt0
+      i_src0 i_tgt0 w0 (st_src0: st_local) (st_tgt0: st_local)
       i_src i_tgt
       (K: _sim_itree sim_itree RR true i_tgt0 w0 (st_src0, i_src) (st_tgt0, i_tgt))
     :
       _sim_itree sim_itree RR i_src0 i_tgt0 w0 (st_src0, tau;; i_src) (st_tgt0, i_tgt)
+
+  | sim_itree_tau_tgt
+      i_src0 i_tgt0 w0 (st_src0: st_local) (st_tgt0: st_local)
+      i_src i_tgt
+      (K: _sim_itree sim_itree RR i_src0 true w0 (st_src0, i_src) (st_tgt0, i_tgt))
+    :
+      _sim_itree sim_itree RR i_src0 i_tgt0 w0 (st_src0, i_src) (st_tgt0, tau;; i_tgt)
+
   | sim_itree_choose_src
-      i_src0 i_tgt0 w0 st_src0 st_tgt0
+      i_src0 i_tgt0 w0 (st_src0: st_local) (st_tgt0: st_local)
       X k_src i_tgt
       (K: exists (x: X), _sim_itree sim_itree RR true i_tgt0 w0 (st_src0, k_src x) (st_tgt0, i_tgt))
     :
       _sim_itree sim_itree RR i_src0 i_tgt0 w0 (st_src0, trigger (Choose X) >>= k_src)
                  (st_tgt0, i_tgt)
+
+  | sim_itree_choose_tgt
+      i_src0 i_tgt0 w0 (st_src0: st_local) (st_tgt0: st_local)
+      X i_src k_tgt
+      (K: forall (x: X), _sim_itree sim_itree RR i_src0 true w0 (st_src0, i_src) (st_tgt0, k_tgt x))
+    :
+      _sim_itree sim_itree RR i_src0 i_tgt0 w0 (st_src0, i_src)
+                 (st_tgt0, trigger (Choose X) >>= k_tgt)
+
   | sim_itree_take_src
-      i_src0 i_tgt0 w0 st_src0 st_tgt0
+      i_src0 i_tgt0 w0 (st_src0: st_local) (st_tgt0: st_local)
       X k_src i_tgt
       (K: forall (x: X), _sim_itree sim_itree RR true i_tgt0 w0 (st_src0, k_src x) (st_tgt0, i_tgt))
     :
       _sim_itree sim_itree RR i_src0 i_tgt0 w0 (st_src0, trigger (Take X) >>= k_src)
                  (st_tgt0, i_tgt)
 
-  | sim_itree_pput_src
-      i_src0 i_tgt0 w0 st_tgt0 st_src0
-      k_src i_tgt
-      st_src1
-      (K: _sim_itree sim_itree RR true i_tgt0 w0 (st_src1, k_src tt) (st_tgt0, i_tgt))
-    :
-      _sim_itree sim_itree RR i_src0 i_tgt0 w0 (st_src0, trigger (PPut st_src1) >>= k_src)
-                 (st_tgt0, i_tgt)
-
-  | sim_itree_pget_src
-      i_src0 i_tgt0 w0 st_tgt0 st_src0
-      k_src i_tgt
-      (K: _sim_itree sim_itree RR true i_tgt0 w0 (st_src0, k_src st_src0) (st_tgt0, i_tgt))
-    :
-      _sim_itree sim_itree RR i_src0 i_tgt0 w0 (st_src0, trigger (PGet) >>= k_src)
-                 (st_tgt0, i_tgt)
-
-
-  | sim_itree_tau_tgt
-      i_src0 i_tgt0 w0 st_src0 st_tgt0
-      i_src i_tgt
-      (K: _sim_itree sim_itree RR i_src0 true w0 (st_src0, i_src) (st_tgt0, i_tgt))
-    :
-      _sim_itree sim_itree RR i_src0 i_tgt0 w0 (st_src0, i_src) (st_tgt0, tau;; i_tgt)
-  | sim_itree_choose_tgt
-      i_src0 i_tgt0 w0 st_src0 st_tgt0
-      X i_src k_tgt
-      (K: forall (x: X), _sim_itree sim_itree RR i_src0 true w0 (st_src0, i_src) (st_tgt0, k_tgt x))
-    :
-      _sim_itree sim_itree RR i_src0 i_tgt0 w0 (st_src0, i_src)
-                 (st_tgt0, trigger (Choose X) >>= k_tgt)
   | sim_itree_take_tgt
-      i_src0 i_tgt0 w0 st_src0 st_tgt0
+      i_src0 i_tgt0 w0 (st_src0: st_local) (st_tgt0: st_local)
       X i_src k_tgt
       (K: exists (x: X), _sim_itree sim_itree RR i_src0 true w0 (st_src0, i_src) (st_tgt0, k_tgt x))
     :
       _sim_itree sim_itree RR i_src0 i_tgt0 w0 (st_src0, i_src)
                  (st_tgt0, trigger (Take X) >>= k_tgt)
 
-  | sim_itree_pput_tgt
-      i_src0 i_tgt0 w0 st_src0 st_tgt0
-      k_tgt i_src
-      st_tgt1
-      (K: _sim_itree sim_itree RR i_src0 true w0 (st_src0, i_src) (st_tgt1, k_tgt tt))
+  | sim_itree_supdate_src
+      i_src0 i_tgt0 w0 (st_src0: st_local) (st_tgt0: st_local)
+      X k_src i_tgt
+      (run: st_local -> st_local * X )
+      (K: _sim_itree sim_itree RR true i_tgt0 w0 (fst (run st_src0), k_src (snd (run st_src0))) (st_tgt0, i_tgt))
     :
-      _sim_itree sim_itree RR i_src0 i_tgt0 w0 (st_src0, i_src)
-                 (st_tgt0, trigger (PPut st_tgt1) >>= k_tgt)
+      _sim_itree sim_itree RR i_src0 i_tgt0 w0 (st_src0, trigger (SUpdate run) >>= k_src) (st_tgt0, i_tgt)  
 
-  | sim_itree_pget_tgt
-      i_src0 i_tgt0 w0 st_src0 st_tgt0
-      k_tgt i_src
-      (K: _sim_itree sim_itree RR i_src0 true w0 (st_src0, i_src) (st_tgt0, k_tgt st_tgt0))
+  | sim_itree_supdate_tgt
+      i_src0 i_tgt0 w0 (st_src0: st_local) (st_tgt0: st_local)
+      X i_src k_tgt
+      (run: st_local -> st_local * X )
+      (K: _sim_itree sim_itree RR i_src0 true w0 (st_src0, i_src) (fst (run st_tgt0), k_tgt (snd (run st_tgt0))))
     :
-      _sim_itree sim_itree RR i_src0 i_tgt0 w0 (st_src0, i_src)
-                 (st_tgt0, trigger (PGet) >>= k_tgt)
+      _sim_itree sim_itree RR i_src0 i_tgt0 w0 (st_src0, i_src) (st_tgt0, trigger (SUpdate run) >>= k_tgt)
 
   | sim_itree_progress
-      i_src0 i_tgt0 w0 st_src0 st_tgt0 i_src i_tgt
+      i_src0 i_tgt0 w0 (st_src0: st_local) (st_tgt0: st_local) i_src i_tgt
       (SIM: sim_itree _ _ RR false false w0 (st_src0, i_src) (st_tgt0, i_tgt))
       (SRC: i_src0 = true)
       (TGT: i_tgt0 = true)
@@ -153,101 +131,86 @@ Section SIM.
   .
 
   Definition lift_rel {R_src R_tgt} (w0: world) (RR: R_src -> R_tgt -> Prop)
-             (st_src st_tgt: st_local) (ret_src ret_tgt : Any.t) :=
+             (st_src0: st_local) (st_tgt0: st_local) (ret_src ret_tgt: Any.t) :=
     exists w1 : world,
-      (<<WLE: le w0 w1 >> /\ <<WF: wf w1 (st_src, st_tgt) >> /\ <<RET: ret_src = ret_tgt >>).
+      (<<WLE: le w0 w1 >> /\ <<WF: wf w1 (st_src0, st_tgt0) >> /\ <<RET: ret_src = ret_tgt >>).
 
-  Lemma _sim_itree_ind2 (sim_itree: forall (R_src R_tgt: Type) (RR: st_local -> st_local -> R_src -> R_tgt -> Prop), bool -> bool -> world -> st_local * itree Es R_src -> st_local * itree Es R_tgt -> Prop)
+  Lemma _sim_itree_ind2 (sim_itree: forall (R_src R_tgt: Type) 
+                                    (RR: st_local -> st_local -> R_src -> R_tgt -> Prop), bool -> bool -> world -> st_local * itree Es R_src -> st_local * itree Es R_tgt -> Prop)
         {R_src R_tgt} (RR: st_local -> st_local -> R_src -> R_tgt -> Prop)
         (P: bool -> bool -> world -> st_local * itree Es R_src -> st_local * itree Es R_tgt -> Prop)
         (RET: forall
             i_src0 i_tgt0 w0 st_src0 st_tgt0
             v_src v_tgt
             (RET: RR st_src0 st_tgt0 v_src v_tgt),
-            P i_src0 i_tgt0 w0 (st_src0, (Ret v_src)) (st_tgt0, (Ret v_tgt)))
+            P i_src0 i_tgt0 w0 (st_src0, Ret v_src) (st_tgt0, Ret v_tgt))
         (CALL: forall
             i_src0 i_tgt0 w w0 st_src0 st_tgt0
             fn varg k_src k_tgt
             (WF: wf w0 (st_src0, st_tgt0))
             (K: forall w1 vret st_src1 st_tgt1 (WLE: le w0 w1) (WF: wf w1 (st_src1, st_tgt1)),
-                sim_itree _ _ RR true true w (st_src1, k_src vret) (st_tgt1, k_tgt vret)),
+                sim_itree _ _ RR false false w (st_src1, k_src vret) (st_tgt1, k_tgt vret)),
             P i_src0 i_tgt0 w (st_src0, trigger (Call fn varg) >>= k_src)
               (st_tgt0, trigger (Call fn varg) >>= k_tgt))
         (SYSCALL: forall
-            i_src0 i_tgt0 w0 st_src0 st_tgt0
+            i_src0 i_tgt0 w0 (st_src0: st_local) (st_tgt0: st_local)
             fn varg rvs k_src k_tgt
             (K: forall vret,
                 sim_itree _ _ RR true true w0 (st_src0, k_src vret) (st_tgt0, k_tgt vret)),
             P i_src0 i_tgt0 w0 (st_src0, trigger (Syscall fn varg rvs) >>= k_src)
               (st_tgt0, trigger (Syscall fn varg rvs) >>= k_tgt))
         (TAUSRC: forall
-            i_src0 i_tgt0 w0 st_src0 st_tgt0
+            i_src0 i_tgt0 w0 (st_src0: st_local) (st_tgt0: st_local)
             i_src i_tgt
             (K: _sim_itree sim_itree RR true i_tgt0 w0 (st_src0, i_src) (st_tgt0, i_tgt))
             (IH: P true i_tgt0 w0 (st_src0, i_src) (st_tgt0, i_tgt)),
             P i_src0 i_tgt0 w0 (st_src0, tau;; i_src) (st_tgt0, i_tgt))
-        (CHOOSESRC: forall
-            i_src0 i_tgt0 w0 st_src0 st_tgt0
-            X k_src i_tgt
-            (K: exists (x: X), <<SIM: _sim_itree sim_itree RR true i_tgt0 w0 (st_src0, k_src x) (st_tgt0, i_tgt)>> /\ <<IH: P true i_tgt0 w0 (st_src0, k_src x) (st_tgt0, i_tgt)>>),
-            P i_src0 i_tgt0 w0 (st_src0, trigger (Choose X) >>= k_src)
-              (st_tgt0, i_tgt))
-        (TAKESRC: forall
-            i_src0 i_tgt0 w0 st_src0 st_tgt0
-            X k_src i_tgt
-            (K: forall (x: X), <<SIM: _sim_itree sim_itree RR true i_tgt0 w0 (st_src0, k_src x) (st_tgt0, i_tgt)>> /\ <<IH: P true i_tgt0 w0 (st_src0, k_src x) (st_tgt0, i_tgt)>>),
-            P i_src0 i_tgt0 w0 (st_src0, trigger (Take X) >>= k_src)
-              (st_tgt0, i_tgt))
-        (PPUTSRC: forall
-            i_src0 i_tgt0 w0 st_tgt0 st_src0
-            k_src i_tgt
-            st_src1
-            (K: _sim_itree sim_itree RR true i_tgt0 w0 (st_src1, k_src tt) (st_tgt0, i_tgt))
-            (IH: P true i_tgt0 w0 (st_src1, k_src tt) (st_tgt0, i_tgt)),
-            P i_src0 i_tgt0 w0 (st_src0, trigger (PPut st_src1) >>= k_src)
-              (st_tgt0, i_tgt))
-        (PGETSRC: forall
-            i_src0 i_tgt0 w0 st_tgt0 st_src0
-            k_src i_tgt
-            (K: _sim_itree sim_itree RR true i_tgt0 w0 (st_src0, k_src st_src0) (st_tgt0, i_tgt))
-            (IH: P true i_tgt0 w0 (st_src0, k_src st_src0) (st_tgt0, i_tgt)),
-            P i_src0 i_tgt0 w0 (st_src0, trigger (PGet) >>= k_src)
-              (st_tgt0, i_tgt))
         (TAUTGT: forall
-            i_src0 i_tgt0 w0 st_src0 st_tgt0
+            i_src0 i_tgt0 w0 (st_src0: st_local) (st_tgt0: st_local)
             i_src i_tgt
             (K: _sim_itree sim_itree RR i_src0 true w0 (st_src0, i_src) (st_tgt0, i_tgt))
             (IH: P i_src0 true w0 (st_src0, i_src) (st_tgt0, i_tgt)),
             P i_src0 i_tgt0 w0 (st_src0, i_src) (st_tgt0, tau;; i_tgt))
+        (CHOOSESRC: forall
+            i_src0 i_tgt0 w0 (st_src0: st_local) (st_tgt0: st_local)
+            X k_src i_tgt
+            (K: exists (x: X), <<SIM: _sim_itree sim_itree RR true i_tgt0 w0 (st_src0, k_src x) (st_tgt0, i_tgt)>> /\ <<IH: P true i_tgt0 w0 (st_src0, k_src x) (st_tgt0, i_tgt)>>),
+            P i_src0 i_tgt0 w0 (st_src0, trigger (Choose X) >>= k_src)
+              (st_tgt0, i_tgt))
         (CHOOSETGT: forall
-            i_src0 i_tgt0 w0 st_src0 st_tgt0
+            i_src0 i_tgt0 w0 (st_src0: st_local) (st_tgt0: st_local)
             X i_src k_tgt
             (K: forall (x: X), <<SIMH: _sim_itree sim_itree RR i_src0 true w0 (st_src0, i_src) (st_tgt0, k_tgt x)>> /\ <<IH: P i_src0 true w0 (st_src0, i_src) (st_tgt0, k_tgt x)>>),
             P i_src0 i_tgt0 w0 (st_src0, i_src)
               (st_tgt0, trigger (Choose X) >>= k_tgt))
+        (TAKESRC: forall
+            i_src0 i_tgt0 w0 (st_src0: st_local) (st_tgt0: st_local)
+            X k_src i_tgt
+            (K: forall (x: X), <<SIM: _sim_itree sim_itree RR true i_tgt0 w0 (st_src0, k_src x) (st_tgt0, i_tgt)>> /\ <<IH: P true i_tgt0 w0 (st_src0, k_src x) (st_tgt0, i_tgt)>>),
+            P i_src0 i_tgt0 w0 (st_src0, trigger (Take X) >>= k_src)
+              (st_tgt0, i_tgt))
         (TAKETGT: forall
-            i_src0 i_tgt0 w0 st_src0 st_tgt0
+            i_src0 i_tgt0 w0 (st_src0: st_local) (st_tgt0: st_local)
             X i_src k_tgt
             (K: exists (x: X), <<SIM:_sim_itree sim_itree RR i_src0 true w0 (st_src0, i_src) (st_tgt0, k_tgt x)>> /\ <<IH: P i_src0 true w0 (st_src0, i_src) (st_tgt0, k_tgt x)>>),
             P i_src0 i_tgt0 w0 (st_src0, i_src)
               (st_tgt0, trigger (Take X) >>= k_tgt))
-        (PPUTTGT: forall
-            i_src0 i_tgt0 w0 st_src0 st_tgt0
-            k_tgt i_src
-            st_tgt1
-            (K: _sim_itree sim_itree RR i_src0 true w0 (st_src0, i_src) (st_tgt1, k_tgt tt))
-            (IH: P i_src0 true w0 (st_src0, i_src) (st_tgt1, k_tgt tt)),
-            P i_src0 i_tgt0 w0 (st_src0, i_src)
-              (st_tgt0, trigger (PPut st_tgt1) >>= k_tgt))
-        (PGETTGT: forall
-            i_src0 i_tgt0 w0 st_src0 st_tgt0
-            k_tgt i_src
-            (K: _sim_itree sim_itree RR i_src0 true w0 (st_src0, i_src) (st_tgt0, k_tgt st_tgt0))
-            (IH: P i_src0 true w0 (st_src0, i_src) (st_tgt0, k_tgt st_tgt0)),
-            P i_src0 i_tgt0 w0 (st_src0, i_src)
-              (st_tgt0, trigger (PGet) >>= k_tgt))
+        (SUPDATESRC: forall
+            i_src0 i_tgt0 w0 (st_src0: st_local) (st_tgt0: st_local)
+            X k_src i_tgt
+            (run: st_local -> st_local * X )
+            (K: _sim_itree sim_itree RR true i_tgt0 w0 (fst (run st_src0), k_src (snd (run st_src0))) (st_tgt0, i_tgt))
+            (IH: P true i_tgt0 w0 (fst (run st_src0), k_src (snd (run st_src0))) (st_tgt0, i_tgt)),
+            P i_src0 i_tgt0 w0 (st_src0, trigger (SUpdate run) >>= k_src) (st_tgt0, i_tgt))
+        (SUPDATETGT: forall
+            i_src0 i_tgt0 w0 (st_src0: st_local) (st_tgt0: st_local)
+            X i_src k_tgt
+            (run: st_local -> st_local * X )
+            (K: _sim_itree sim_itree RR i_src0 true w0 (st_src0, i_src) (fst (run st_tgt0), k_tgt (snd (run st_tgt0))))
+            (IH: P i_src0 true w0 (st_src0, i_src) (fst (run st_tgt0), k_tgt (snd (run st_tgt0)))),
+            P i_src0 i_tgt0 w0 (st_src0, i_src) (st_tgt0, trigger (SUpdate run) >>= k_tgt))
         (PROGRESS: forall
-            i_src0 i_tgt0 w0 st_src0 st_tgt0 i_src i_tgt
+            i_src0 i_tgt0 w0 (st_src0: st_local) (st_tgt0: st_local) i_src i_tgt
             (SIM: sim_itree _ _ RR false false w0 (st_src0, i_src) (st_tgt0, i_tgt))
             (SRC: i_src0 = true)
             (TGT: i_tgt0 = true),
@@ -262,19 +225,18 @@ Section SIM.
     { eapply CALL; eauto. }
     { eapply SYSCALL; eauto. }
     { eapply TAUSRC; eauto. }
-    { eapply CHOOSESRC; eauto. des. esplits; eauto. }
-    { eapply TAKESRC; eauto. }
-    { eapply PPUTSRC; eauto. }
-    { eapply PGETSRC; eauto. }
     { eapply TAUTGT; eauto. }
+    { eapply CHOOSESRC; eauto. des. esplits; eauto. }
     { eapply CHOOSETGT; eauto. }
+    { eapply TAKESRC; eauto. }
     { eapply TAKETGT; eauto. des. esplits; eauto. }
-    { eapply PPUTTGT; eauto. }
-    { eapply PGETTGT; eauto. }
+    { eapply SUPDATESRC; eauto. }
+    { eapply SUPDATETGT; eauto. }
     { eapply PROGRESS; eauto. }
+
   Qed.
 
-  Definition sim_itree o_src o_tgt w0: relation _ :=
+  Definition sim_itree o_src o_tgt w0 : relation _ :=
     paco8 _sim_itree bot8 _ _ (lift_rel w0 (@eq Any.t)) o_src o_tgt w0.
 
   Lemma sim_itree_mon: monotone8 _sim_itree.
@@ -290,96 +252,82 @@ Section SIM.
   Hint Resolve cpn8_wcompat: paco.
 
   Lemma sim_itree_ind
-        R_src R_tgt (RR: st_local -> st_local -> R_src -> R_tgt -> Prop)
+        R_src R_tgt (RR: st_local -> st_local -> R_src -> R_tgt -> Prop) 
         (P: bool -> bool -> world -> st_local * itree Es R_src -> st_local * itree Es R_tgt -> Prop)
         (RET: forall
             i_src0 i_tgt0 w0 st_src0 st_tgt0
             v_src v_tgt
             (RET: RR st_src0 st_tgt0 v_src v_tgt),
-            P i_src0 i_tgt0 w0 (st_src0, (Ret v_src)) (st_tgt0, (Ret v_tgt)))
+            P i_src0 i_tgt0 w0 (st_src0, Ret v_src) (st_tgt0, Ret v_tgt))
         (CALL: forall
             i_src0 i_tgt0 w w0 st_src0 st_tgt0
             fn varg k_src k_tgt
             (WF: wf w0 (st_src0, st_tgt0))
             (K: forall w1 vret st_src1 st_tgt1 (WLE: le w0 w1) (WF: wf w1 (st_src1, st_tgt1)),
-                paco8 _sim_itree bot8 _ _ RR true true w (st_src1, k_src vret) (st_tgt1, k_tgt vret)),
+                paco8 _sim_itree bot8 _ _ RR false false w (st_src1, k_src vret) (st_tgt1, k_tgt vret)),
             P i_src0 i_tgt0 w (st_src0, trigger (Call fn varg) >>= k_src)
               (st_tgt0, trigger (Call fn varg) >>= k_tgt))
         (SYSCALL: forall
-            i_src0 i_tgt0 w0 st_src0 st_tgt0
+            i_src0 i_tgt0 w0 (st_src0: st_local) (st_tgt0: st_local)
             fn varg rvs k_src k_tgt
             (K: forall vret,
                 paco8 _sim_itree bot8 _ _ RR true true w0 (st_src0, k_src vret) (st_tgt0, k_tgt vret)),
             P i_src0 i_tgt0 w0 (st_src0, trigger (Syscall fn varg rvs) >>= k_src)
               (st_tgt0, trigger (Syscall fn varg rvs) >>= k_tgt))
         (TAUSRC: forall
-            i_src0 i_tgt0 w0 st_src0 st_tgt0
+            i_src0 i_tgt0 w0 (st_src0: st_local) (st_tgt0: st_local)
             i_src i_tgt
             (K: paco8 _sim_itree bot8 _ _ RR true i_tgt0 w0 (st_src0, i_src) (st_tgt0, i_tgt))
             (IH: P true i_tgt0 w0 (st_src0, i_src) (st_tgt0, i_tgt)),
             P i_src0 i_tgt0 w0 (st_src0, tau;; i_src) (st_tgt0, i_tgt))
+        (TAUTGT: forall
+            i_src0 i_tgt0 w0 (st_src0: st_local) (st_tgt0: st_local)
+            i_src i_tgt
+            (K: paco8 _sim_itree bot8 _ _ RR i_src0 true w0 (st_src0, i_src) (st_tgt0, i_tgt))
+            (IH: P i_src0 true w0 (st_src0, i_src) (st_tgt0, i_tgt)),
+            P i_src0 i_tgt0 w0 (st_src0, i_src) (st_tgt0, tau;; i_tgt))            
         (CHOOSESRC: forall
-            i_src0 i_tgt0 w0 st_src0 st_tgt0
+            i_src0 i_tgt0 w0 (st_src0: st_local) (st_tgt0: st_local)
             X k_src i_tgt
             (K: exists (x: X), <<SIM: paco8 _sim_itree bot8 _ _ RR true i_tgt0 w0 (st_src0, k_src x) (st_tgt0, i_tgt)>> /\ <<IH: P true i_tgt0 w0 (st_src0, k_src x) (st_tgt0, i_tgt)>>),
             P i_src0 i_tgt0 w0 (st_src0, trigger (Choose X) >>= k_src)
               (st_tgt0, i_tgt))
-        (TAKESRC: forall
-            i_src0 i_tgt0 w0 st_src0 st_tgt0
-            X k_src i_tgt
-            (K: forall (x: X), <<SIM: paco8 _sim_itree bot8 _ _ RR true i_tgt0 w0 (st_src0, k_src x) (st_tgt0, i_tgt)>> /\ <<IH: P true i_tgt0 w0 (st_src0, k_src x) (st_tgt0, i_tgt)>>),
-            P i_src0 i_tgt0 w0 (st_src0, trigger (Take X) >>= k_src)
-              (st_tgt0, i_tgt))
-        (PPUTSRC: forall
-            i_src0 i_tgt0 w0 st_tgt0 st_src0
-            k_src i_tgt
-            st_src1
-            (K: paco8 _sim_itree bot8 _ _ RR true i_tgt0 w0 (st_src1, k_src tt) (st_tgt0, i_tgt))
-            (IH: P true i_tgt0 w0 (st_src1, k_src tt) (st_tgt0, i_tgt)),
-            P i_src0 i_tgt0 w0 (st_src0, trigger (PPut st_src1) >>= k_src)
-              (st_tgt0, i_tgt))
-        (PGETSRC: forall
-            i_src0 i_tgt0 w0 st_tgt0 st_src0
-            k_src i_tgt
-            (K: paco8 _sim_itree bot8 _ _ RR true i_tgt0 w0 (st_src0, k_src st_src0) (st_tgt0, i_tgt))
-            (IH: P true i_tgt0 w0 (st_src0, k_src st_src0) (st_tgt0, i_tgt)),
-            P i_src0 i_tgt0 w0 (st_src0, trigger (PGet) >>= k_src)
-              (st_tgt0, i_tgt))
-        (TAUTGT: forall
-            i_src0 i_tgt0 w0 st_src0 st_tgt0
-            i_src i_tgt
-            (K: paco8 _sim_itree bot8 _ _ RR i_src0 true w0 (st_src0, i_src) (st_tgt0, i_tgt))
-            (IH: P i_src0 true w0 (st_src0, i_src) (st_tgt0, i_tgt)),
-            P i_src0 i_tgt0 w0 (st_src0, i_src) (st_tgt0, tau;; i_tgt))
         (CHOOSETGT: forall
-            i_src0 i_tgt0 w0 st_src0 st_tgt0
+            i_src0 i_tgt0 w0 (st_src0: st_local) (st_tgt0: st_local)
             X i_src k_tgt
             (K: forall (x: X), <<SIMH: paco8 _sim_itree bot8 _ _ RR i_src0 true w0 (st_src0, i_src) (st_tgt0, k_tgt x)>> /\ <<IH: P i_src0 true w0 (st_src0, i_src) (st_tgt0, k_tgt x)>>),
             P i_src0 i_tgt0 w0 (st_src0, i_src)
               (st_tgt0, trigger (Choose X) >>= k_tgt))
+        (TAKESRC: forall
+            i_src0 i_tgt0 w0 (st_src0: st_local) (st_tgt0: st_local)
+            X k_src i_tgt
+            (K: forall (x: X), <<SIM: paco8 _sim_itree bot8 _ _ RR true i_tgt0 w0 (st_src0, k_src x) (st_tgt0, i_tgt)>> /\ <<IH: P true i_tgt0 w0 (st_src0, k_src x) (st_tgt0, i_tgt)>>),
+            P i_src0 i_tgt0 w0 (st_src0, trigger (Take X) >>= k_src)
+              (st_tgt0, i_tgt))
         (TAKETGT: forall
-            i_src0 i_tgt0 w0 st_src0 st_tgt0
+            i_src0 i_tgt0 w0 (st_src0: st_local) (st_tgt0: st_local)
             X i_src k_tgt
             (K: exists (x: X), <<SIM:paco8 _sim_itree bot8 _ _ RR i_src0 true w0 (st_src0, i_src) (st_tgt0, k_tgt x)>> /\ <<IH: P i_src0 true w0 (st_src0, i_src) (st_tgt0, k_tgt x)>>),
             P i_src0 i_tgt0 w0 (st_src0, i_src)
               (st_tgt0, trigger (Take X) >>= k_tgt))
-        (PPUTTGT: forall
-            i_src0 i_tgt0 w0 st_src0 st_tgt0
-            k_tgt i_src
-            st_tgt1
-            (K: paco8 _sim_itree bot8 _ _ RR i_src0 true w0 (st_src0, i_src) (st_tgt1, k_tgt tt))
-            (IH: P i_src0 true w0 (st_src0, i_src) (st_tgt1, k_tgt tt)),
-            P i_src0 i_tgt0 w0 (st_src0, i_src)
-              (st_tgt0, trigger (PPut st_tgt1) >>= k_tgt))
-        (PGETTGT: forall
-            i_src0 i_tgt0 w0 st_src0 st_tgt0
-            k_tgt i_src
-            (K: paco8 _sim_itree bot8 _ _ RR i_src0 true w0 (st_src0, i_src) (st_tgt0, k_tgt st_tgt0))
-            (IH: P i_src0 true w0 (st_src0, i_src) (st_tgt0, k_tgt st_tgt0)),
-            P i_src0 i_tgt0 w0 (st_src0, i_src)
-              (st_tgt0, trigger (PGet) >>= k_tgt))
+        (SUPDATESRC: forall
+            i_src0 i_tgt0 w0 (st_src0: st_local) (st_tgt0: st_local)
+            X k_src i_tgt
+            (run: st_local -> st_local * X )
+            (K: paco8 _sim_itree bot8 _ _ RR true i_tgt0 w0 (fst (run st_src0), k_src (snd (run st_src0))) (st_tgt0, i_tgt))
+            (IH: P true i_tgt0 w0 (fst (run st_src0), k_src (snd (run st_src0))) (st_tgt0, i_tgt)),
+            P i_src0 i_tgt0 w0 (st_src0, trigger (SUpdate run) >>= k_src) (st_tgt0, i_tgt))
+        (SUPDATETGT: forall
+            i_src0 i_tgt0 w0 (st_src0: st_local) (st_tgt0: st_local)
+            X i_src k_tgt
+            (run: st_local -> st_local * X )
+            (K: paco8 _sim_itree bot8 _ _ RR i_src0 true w0 (st_src0, i_src) (fst (run st_tgt0), k_tgt (snd (run st_tgt0))))
+            (IH:  P i_src0 true w0 (st_src0, i_src) (fst (run st_tgt0), k_tgt (snd (run st_tgt0)))),
+
+            P i_src0 i_tgt0 w0 (st_src0, i_src) (st_tgt0, trigger (SUpdate run) >>= k_tgt))       
         (PROGRESS: forall
-            i_src0 i_tgt0 w0 st_src0 st_tgt0 i_src i_tgt
+            i_src0 i_tgt0 w0 (st_src0: st_local) (st_tgt0: st_local)
+            i_src i_tgt
             (SIM: paco8 _sim_itree bot8 _ _ RR false false w0 (st_src0, i_src) (st_tgt0, i_tgt))
             (SRC: i_src0 = true)
             (TGT: i_tgt0 = true),
@@ -394,18 +342,17 @@ Section SIM.
     { eapply CALL; eauto. i. exploit K; eauto. i. pclearbot. eauto. }
     { eapply SYSCALL; eauto. i. exploit K; eauto. i. pclearbot. eauto. }
     { eapply TAUSRC; eauto. }
+    { eapply TAUTGT; eauto. }
     { eapply CHOOSESRC; eauto. des. esplits; eauto. }
+    { eapply CHOOSETGT; eauto. i. exploit K; eauto. i. des.
+    pclearbot. esplits; eauto. }
     { eapply TAKESRC; eauto. i. exploit K; eauto. i. des.
       pclearbot. esplits; eauto. }
-    { eapply PPUTSRC; eauto. }
-    { eapply PGETSRC; eauto. }
-    { eapply TAUTGT; eauto. }
-    { eapply CHOOSETGT; eauto. i. exploit K; eauto. i. des.
-      pclearbot. esplits; eauto. }
     { eapply TAKETGT; eauto. des. esplits; eauto. }
-    { eapply PPUTTGT; eauto. }
-    { eapply PGETTGT; eauto. }
+    { eapply SUPDATESRC; eauto. }
+    { eapply SUPDATETGT; eauto. }
     { eapply PROGRESS; eauto. pclearbot. auto. }
+
   Qed.
 
   Variant sim_itree_indC (sim_itree: forall (R_src R_tgt: Type) (RR: st_local -> st_local -> R_src -> R_tgt -> Prop), bool -> bool -> world -> st_local * itree Es R_src -> st_local * itree Es R_tgt -> Prop)
@@ -416,101 +363,84 @@ Section SIM.
       v_src v_tgt
       (RET: RR st_src0 st_tgt0 v_src v_tgt)
     :
-      sim_itree_indC sim_itree RR i_src0 i_tgt0 w0 (st_src0, (Ret v_src)) (st_tgt0, (Ret v_tgt))
+      sim_itree_indC  sim_itree RR i_src0 i_tgt0 w0 (st_src0, Ret v_src) (st_tgt0, Ret v_tgt)
   | sim_itree_indC_call
       i_src0 i_tgt0 w w0 st_src0 st_tgt0
       fn varg k_src k_tgt
       (WF: wf w0 (st_src0, st_tgt0))
       (K: forall w1 vret st_src1 st_tgt1 (WLE: le w0 w1) (WF: wf w1 (st_src1, st_tgt1)),
-          sim_itree _ _ RR true true w (st_src1, k_src vret) (st_tgt1, k_tgt vret))
+          sim_itree _ _ RR false false w (st_src1, k_src vret) (st_tgt1, k_tgt vret))
     :
-      sim_itree_indC sim_itree RR i_src0 i_tgt0 w (st_src0, trigger (Call fn varg) >>= k_src)
+      sim_itree_indC  sim_itree RR i_src0 i_tgt0 w (st_src0, trigger (Call fn varg) >>= k_src)
                      (st_tgt0, trigger (Call fn varg) >>= k_tgt)
   | sim_itree_indC_syscall
-      i_src0 i_tgt0 w0 st_src0 st_tgt0
+      i_src0 i_tgt0 w0 (st_src0: st_local) (st_tgt0: st_local)
       fn varg rvs k_src k_tgt
       (K: forall vret,
           sim_itree _ _ RR true true w0 (st_src0, k_src vret) (st_tgt0, k_tgt vret))
     :
-      sim_itree_indC sim_itree RR i_src0 i_tgt0 w0 (st_src0, trigger (Syscall fn varg rvs) >>= k_src)
+      sim_itree_indC  sim_itree RR i_src0 i_tgt0 w0 (st_src0, trigger (Syscall fn varg rvs) >>= k_src)
                      (st_tgt0, trigger (Syscall fn varg rvs) >>= k_tgt)
 
   | sim_itree_indC_tau_src
-      i_src0 i_tgt0 w0 st_src0 st_tgt0
+      i_src0 i_tgt0 w0 (st_src0: st_local) (st_tgt0: st_local)
       i_src i_tgt
       (K: sim_itree _ _ RR true i_tgt0 w0 (st_src0, i_src) (st_tgt0, i_tgt))
     :
-      sim_itree_indC sim_itree RR i_src0 i_tgt0 w0 (st_src0, tau;; i_src) (st_tgt0, i_tgt)
-  | sim_itree_indC_choose_src
-      i_src0 i_tgt0 w0 st_src0 st_tgt0
-      X k_src i_tgt
-      (K: exists (x: X), sim_itree _ _ RR true i_tgt0 w0 (st_src0, k_src x) (st_tgt0, i_tgt))
-    :
-      sim_itree_indC sim_itree RR i_src0 i_tgt0 w0 (st_src0, trigger (Choose X) >>= k_src)
-                     (st_tgt0, i_tgt)
-  | sim_itree_indC_take_src
-      i_src0 i_tgt0 w0 st_src0 st_tgt0
-      X k_src i_tgt
-      (K: forall (x: X), sim_itree _ _ RR true i_tgt0 w0 (st_src0, k_src x) (st_tgt0, i_tgt))
-    :
-      sim_itree_indC sim_itree RR i_src0 i_tgt0 w0 (st_src0, trigger (Take X) >>= k_src)
-                     (st_tgt0, i_tgt)
-
-  | sim_itree_indC_pput_src
-      i_src0 i_tgt0 w0 st_tgt0 st_src0
-      k_src i_tgt
-      st_src1
-      (K: sim_itree _ _ RR true i_tgt0 w0 (st_src1, k_src tt) (st_tgt0, i_tgt))
-    :
-      sim_itree_indC sim_itree RR i_src0 i_tgt0 w0 (st_src0, trigger (PPut st_src1) >>= k_src)
-                     (st_tgt0, i_tgt)
-
-  | sim_itree_indC_pget_src
-      i_src0 i_tgt0 w0 st_tgt0 st_src0
-      k_src i_tgt
-      (K: sim_itree _ _ RR true i_tgt0 w0 (st_src0, k_src st_src0) (st_tgt0, i_tgt))
-    :
-      sim_itree_indC sim_itree RR i_src0 i_tgt0 w0 (st_src0, trigger (PGet) >>= k_src)
-                     (st_tgt0, i_tgt)
-
+      sim_itree_indC  sim_itree RR i_src0 i_tgt0 w0 (st_src0, tau;; i_src) (st_tgt0, i_tgt)
 
   | sim_itree_indC_tau_tgt
-      i_src0 i_tgt0 w0 st_src0 st_tgt0
+      i_src0 i_tgt0 w0 (st_src0: st_local) (st_tgt0: st_local)
       i_src i_tgt
       (K: sim_itree _ _ RR i_src0 true w0 (st_src0, i_src) (st_tgt0, i_tgt))
     :
-      sim_itree_indC sim_itree RR i_src0 i_tgt0 w0 (st_src0, i_src) (st_tgt0, tau;; i_tgt)
+      sim_itree_indC  sim_itree RR i_src0 i_tgt0 w0 (st_src0, i_src) (st_tgt0, tau;; i_tgt)
+
+  | sim_itree_indC_choose_src
+      i_src0 i_tgt0 w0 (st_src0: st_local) (st_tgt0: st_local)
+      X k_src i_tgt
+      (K: exists (x: X), sim_itree _ _ RR true i_tgt0 w0 (st_src0, k_src x) (st_tgt0, i_tgt))
+    :
+      sim_itree_indC  sim_itree RR i_src0 i_tgt0 w0 (st_src0, trigger (Choose X) >>= k_src)
+                     (st_tgt0, i_tgt)
   | sim_itree_indC_choose_tgt
-      i_src0 i_tgt0 w0 st_src0 st_tgt0
+      i_src0 i_tgt0 w0 (st_src0: st_local) (st_tgt0: st_local)
       X i_src k_tgt
       (K: forall (x: X), sim_itree _ _ RR i_src0 true w0 (st_src0, i_src) (st_tgt0, k_tgt x))
     :
-      sim_itree_indC sim_itree RR i_src0 i_tgt0 w0 (st_src0, i_src)
+      sim_itree_indC  sim_itree RR i_src0 i_tgt0 w0 (st_src0, i_src)
                      (st_tgt0, trigger (Choose X) >>= k_tgt)
+
+  | sim_itree_indC_take_src
+      i_src0 i_tgt0 w0 (st_src0: st_local) (st_tgt0: st_local)
+      X k_src i_tgt
+      (K: forall (x: X), sim_itree _ _ RR true i_tgt0 w0 (st_src0, k_src x) (st_tgt0, i_tgt))
+    :
+      sim_itree_indC  sim_itree RR i_src0 i_tgt0 w0 (st_src0, trigger (Take X) >>= k_src)
+                     (st_tgt0, i_tgt)
   | sim_itree_indC_take_tgt
-      i_src0 i_tgt0 w0 st_src0 st_tgt0
+      i_src0 i_tgt0 w0 (st_src0: st_local) (st_tgt0: st_local)
       X i_src k_tgt
       (K: exists (x: X), sim_itree _ _ RR i_src0 true w0 (st_src0, i_src) (st_tgt0, k_tgt x))
     :
-      sim_itree_indC sim_itree RR i_src0 i_tgt0 w0 (st_src0, i_src)
+      sim_itree_indC  sim_itree RR i_src0 i_tgt0 w0 (st_src0, i_src)
                      (st_tgt0, trigger (Take X) >>= k_tgt)
-
-  | sim_itree_indC_pput_tgt
-      i_src0 i_tgt0 w0 st_src0 st_tgt0
-      k_tgt i_src
-      st_tgt1
-      (K: sim_itree _ _ RR i_src0 true w0 (st_src0, i_src) (st_tgt1, k_tgt tt))
+  
+  | sim_itree_indC_supdate_src
+      i_src0 i_tgt0 w0 (st_src0: st_local) (st_tgt0: st_local)
+      X k_src i_tgt
+      (run: st_local -> st_local * X )
+      (K: sim_itree _ _ RR true i_tgt0 w0 (fst (run st_src0), k_src (snd (run st_src0))) (st_tgt0, i_tgt))
     :
-      sim_itree_indC sim_itree RR i_src0 i_tgt0 w0 (st_src0, i_src)
-                     (st_tgt0, trigger (PPut st_tgt1) >>= k_tgt)
+      sim_itree_indC  sim_itree RR i_src0 i_tgt0 w0 (st_src0, trigger (SUpdate run) >>= k_src) (st_tgt0, i_tgt)
 
-  | sim_itree_indC_pget_tgt
-      i_src0 i_tgt0 w0 st_src0 st_tgt0
-      k_tgt i_src
-      (K: sim_itree _ _ RR i_src0 true w0 (st_src0, i_src) (st_tgt0, k_tgt st_tgt0))
+  | sim_itree_indC_supdate_tgt
+      i_src0 i_tgt0 w0 (st_src0: st_local) (st_tgt0: st_local)
+      X i_src k_tgt
+      (run: st_local -> st_local * X )
+      (K: sim_itree _ _ RR i_src0 true w0 (st_src0, i_src) (fst (run st_tgt0), k_tgt (snd (run st_tgt0))))
     :
-      sim_itree_indC sim_itree RR i_src0 i_tgt0 w0 (st_src0, i_src)
-                     (st_tgt0, trigger (PGet) >>= k_tgt)
+      sim_itree_indC  sim_itree RR i_src0 i_tgt0 w0 (st_src0, i_src) (st_tgt0, trigger (SUpdate run) >>= k_tgt)
   .
 
   Lemma sim_itree_indC_mon: monotone8 sim_itree_indC.
@@ -529,15 +459,13 @@ Section SIM.
       esplits; eauto. eapply rclo8_base. eauto. }
     { econs 3; eauto. i. eapply rclo8_base. eauto. }
     { econs 4; eauto. eapply sim_itree_mon; eauto. i. eapply rclo8_base. eauto. }
-    { econs 5; eauto. des. esplits; eauto. eapply sim_itree_mon; eauto. i. eapply rclo8_base. eauto. }
-    { econs 6; eauto. i. eapply sim_itree_mon; eauto. i. eapply rclo8_base. eauto. }
-    { econs 7; eauto. eapply sim_itree_mon; eauto. i. eapply rclo8_base. eauto. }
-    { econs 8; eauto. eapply sim_itree_mon; eauto. i. eapply rclo8_base. eauto. }
-    { econs 9; eauto. eapply sim_itree_mon; eauto. i. eapply rclo8_base. eauto. }
-    { econs 10; eauto. i. eapply sim_itree_mon; eauto. i. eapply rclo8_base. eauto. }
-    { econs 11; eauto. des. esplits; eauto. eapply sim_itree_mon; eauto. i. eapply rclo8_base. eauto. }
-    { econs 12; eauto. eapply sim_itree_mon; eauto. i. eapply rclo8_base. eauto. }
-    { econs 13; eauto. eapply sim_itree_mon; eauto. i. eapply rclo8_base. eauto. }
+    { econs 5; eauto. eapply sim_itree_mon; eauto. i. eapply rclo8_base. eauto. }
+    { econs 6; eauto. des. esplits; eauto. eapply sim_itree_mon; eauto. i. eapply rclo8_base. eauto. }
+    { econs 7; eauto. i. eapply sim_itree_mon; eauto. i. eapply rclo8_base. eauto. }
+    { econs 8; eauto. i. eapply sim_itree_mon; eauto. i. eapply rclo8_base. eauto. }
+    { econs 9; eauto. des. esplits; eauto. eapply sim_itree_mon; eauto. i. eapply rclo8_base. eauto. }
+    { econs 10; eauto. des. esplits; eauto. eapply sim_itree_mon; eauto. i. eapply rclo8_base. eauto.  }
+    { econs 11; eauto. des. esplits; eauto.  eapply sim_itree_mon; eauto. i. eapply rclo8_base. eauto.  }
   Qed.
 
   Variant sim_itreeC (r g: forall (R_src R_tgt: Type) (RR: st_local -> st_local -> R_src -> R_tgt -> Prop), bool -> bool -> world -> st_local * itree Es R_src -> st_local * itree Es R_tgt -> Prop)
@@ -548,18 +476,18 @@ Section SIM.
       v_src v_tgt
       (RET: RR st_src0 st_tgt0 v_src v_tgt)
     :
-      sim_itreeC r g RR i_src0 i_tgt0 w0 (st_src0, (Ret v_src)) (st_tgt0, (Ret v_tgt))
+      sim_itreeC r g RR i_src0 i_tgt0 w0 (st_src0, Ret v_src) (st_tgt0, Ret v_tgt)
   | sim_itreeC_call
       i_src0 i_tgt0 w w0 st_src0 st_tgt0
       fn varg k_src k_tgt
       (WF: wf w0 (st_src0, st_tgt0))
       (K: forall w1 vret st_src1 st_tgt1 (WLE: le w0 w1) (WF: wf w1 (st_src1, st_tgt1)),
-          g _ _ RR true true w (st_src1, k_src vret) (st_tgt1, k_tgt vret))
+          g _ _ RR false false w (st_src1, k_src vret) (st_tgt1, k_tgt vret))
     :
       sim_itreeC r g RR i_src0 i_tgt0 w (st_src0, trigger (Call fn varg) >>= k_src)
                  (st_tgt0, trigger (Call fn varg) >>= k_tgt)
   | sim_itreeC_syscall
-      i_src0 i_tgt0 w0 st_src0 st_tgt0
+      i_src0 i_tgt0 w0 (st_src0: st_local) (st_tgt0: st_local)
       fn varg rvs k_src k_tgt
       (K: forall vret,
           g _ _ RR true true w0 (st_src0, k_src vret) (st_tgt0, k_tgt vret))
@@ -568,81 +496,64 @@ Section SIM.
                  (st_tgt0, trigger (Syscall fn varg rvs) >>= k_tgt)
 
   | sim_itreeC_tau_src
-      i_src0 i_tgt0 w0 st_src0 st_tgt0
+      i_src0 i_tgt0 w0 (st_src0: st_local) (st_tgt0: st_local)
       i_src i_tgt
       (K: r _ _ RR true i_tgt0 w0 (st_src0, i_src) (st_tgt0, i_tgt))
     :
       sim_itreeC r g RR i_src0 i_tgt0 w0 (st_src0, tau;; i_src) (st_tgt0, i_tgt)
+
+  | sim_itreeC_tau_tgt
+      i_src0 i_tgt0 w0 (st_src0: st_local) (st_tgt0: st_local)
+      i_src i_tgt
+      (K: r _ _ RR i_src0 true w0 (st_src0, i_src) (st_tgt0, i_tgt))
+    :
+      sim_itreeC r g RR i_src0 i_tgt0 w0 (st_src0, i_src) (st_tgt0, tau;; i_tgt)
+
+
   | sim_itreeC_choose_src
-      i_src0 i_tgt0 w0 st_src0 st_tgt0
+      i_src0 i_tgt0 w0 (st_src0: st_local) (st_tgt0: st_local)
       X k_src i_tgt
       (K: exists (x: X), r _ _ RR true i_tgt0 w0 (st_src0, k_src x) (st_tgt0, i_tgt))
     :
       sim_itreeC r g RR i_src0 i_tgt0 w0 (st_src0, trigger (Choose X) >>= k_src)
                  (st_tgt0, i_tgt)
-  | sim_itreeC_take_src
-      i_src0 i_tgt0 w0 st_src0 st_tgt0
-      X k_src i_tgt
-      (K: forall (x: X), r _ _ RR true i_tgt0 w0 (st_src0, k_src x) (st_tgt0, i_tgt))
-    :
-      sim_itreeC r g RR i_src0 i_tgt0 w0 (st_src0, trigger (Take X) >>= k_src)
-                 (st_tgt0, i_tgt)
-
-  | sim_itreeC_pput_src
-      i_src0 i_tgt0 w0 st_tgt0 st_src0
-      k_src i_tgt
-      st_src1
-      (K: r _ _ RR true i_tgt0 w0 (st_src1, k_src tt) (st_tgt0, i_tgt))
-    :
-      sim_itreeC r g RR i_src0 i_tgt0 w0 (st_src0, trigger (PPut st_src1) >>= k_src)
-                 (st_tgt0, i_tgt)
-
-  | sim_itreeC_pget_src
-      i_src0 i_tgt0 w0 st_tgt0 st_src0
-      k_src i_tgt
-      (K: r _ _ RR true i_tgt0 w0 (st_src0, k_src st_src0) (st_tgt0, i_tgt))
-    :
-      sim_itreeC r g RR i_src0 i_tgt0 w0 (st_src0, trigger (PGet) >>= k_src)
-                 (st_tgt0, i_tgt)
-
-
-  | sim_itreeC_tau_tgt
-      i_src0 i_tgt0 w0 st_src0 st_tgt0
-      i_src i_tgt
-      (K: r _ _ RR i_src0 true w0 (st_src0, i_src) (st_tgt0, i_tgt))
-    :
-      sim_itreeC r g RR i_src0 i_tgt0 w0 (st_src0, i_src) (st_tgt0, tau;; i_tgt)
   | sim_itreeC_choose_tgt
-      i_src0 i_tgt0 w0 st_src0 st_tgt0
+      i_src0 i_tgt0 w0 (st_src0: st_local) (st_tgt0: st_local)
       X i_src k_tgt
       (K: forall (x: X), r _ _ RR i_src0 true w0 (st_src0, i_src) (st_tgt0, k_tgt x))
     :
       sim_itreeC r g RR i_src0 i_tgt0 w0 (st_src0, i_src)
                  (st_tgt0, trigger (Choose X) >>= k_tgt)
+  | sim_itreeC_take_src
+      i_src0 i_tgt0 w0 (st_src0: st_local) (st_tgt0: st_local)
+      X k_src i_tgt
+      (K: forall (x: X), r _ _ RR true i_tgt0 w0 (st_src0, k_src x) (st_tgt0, i_tgt))
+    :
+      sim_itreeC r g RR i_src0 i_tgt0 w0 (st_src0, trigger (Take X) >>= k_src)
+                 (st_tgt0, i_tgt)
   | sim_itreeC_take_tgt
-      i_src0 i_tgt0 w0 st_src0 st_tgt0
+      i_src0 i_tgt0 w0 (st_src0: st_local) (st_tgt0: st_local)
       X i_src k_tgt
       (K: exists (x: X), r _ _ RR i_src0 true w0 (st_src0, i_src) (st_tgt0, k_tgt x))
     :
       sim_itreeC r g RR i_src0 i_tgt0 w0 (st_src0, i_src)
                  (st_tgt0, trigger (Take X) >>= k_tgt)
-
-  | sim_itreeC_pput_tgt
-      i_src0 i_tgt0 w0 st_src0 st_tgt0
-      k_tgt i_src
-      st_tgt1
-      (K: r _ _ RR i_src0 true w0 (st_src0, i_src) (st_tgt1, k_tgt tt))
+  | sim_itreeC_supdate_src
+      i_src0 i_tgt0 w0 (st_src0: st_local) (st_tgt0: st_local)
+      X k_src i_tgt
+      (run: st_local -> st_local * X )
+      (K: r _ _ RR true i_tgt0 w0 (fst (run st_src0), k_src (snd (run st_src0))) (st_tgt0, i_tgt))
     :
-      sim_itreeC r g RR i_src0 i_tgt0 w0 (st_src0, i_src)
-                 (st_tgt0, trigger (PPut st_tgt1) >>= k_tgt)
+      sim_itreeC r g RR i_src0 i_tgt0 w0 (st_src0, trigger (SUpdate run) >>= k_src) (st_tgt0, i_tgt)
 
-  | sim_itreeC_pget_tgt
-      i_src0 i_tgt0 w0 st_src0 st_tgt0
-      k_tgt i_src
-      (K: r _ _ RR i_src0 true w0 (st_src0, i_src) (st_tgt0, k_tgt st_tgt0))
+  | sim_itreeC_supdate_tgt
+      i_src0 i_tgt0 w0 (st_src0: st_local) (st_tgt0: st_local)
+      X i_src k_tgt
+      (run: st_local -> st_local * X )
+      (K: r _ _ RR i_src0 true w0 (st_src0, i_src) (fst (run st_tgt0), k_tgt (snd (run st_tgt0))))
     :
-      sim_itreeC r g RR i_src0 i_tgt0 w0 (st_src0, i_src)
-                 (st_tgt0, trigger (PGet) >>= k_tgt)
+      sim_itreeC r g RR i_src0 i_tgt0 w0 (st_src0, i_src) (st_tgt0, trigger (SUpdate run) >>= k_tgt)
+
   .
 
   Lemma sim_itreeC_spec_aux:
@@ -653,15 +564,13 @@ Section SIM.
     { gstep. econs 2; eauto. i. gbase. eauto. }
     { gstep. econs 3; eauto. i. gbase. eauto. }
     { guclo sim_itree_indC_spec. econs 4; eauto. gbase. eauto. }
-    { guclo sim_itree_indC_spec. econs 5; eauto. des. esplits; eauto. gbase. eauto. }
-    { guclo sim_itree_indC_spec. econs 6; eauto. i. gbase. eauto. }
+    { guclo sim_itree_indC_spec. econs 5; eauto. gbase. eauto. }
+    { guclo sim_itree_indC_spec. econs 6; eauto. des. esplits; eauto. gbase. eauto. }
     { guclo sim_itree_indC_spec. econs 7; eauto. gbase. eauto. }
     { guclo sim_itree_indC_spec. econs 8; eauto. gbase. eauto. }
-    { guclo sim_itree_indC_spec. econs 9; eauto. gbase. eauto. }
-    { guclo sim_itree_indC_spec. econs 10; eauto. i. gbase. eauto. }
-    { guclo sim_itree_indC_spec. econs 11; eauto. des. esplits; eauto. gbase. eauto. }
-    { guclo sim_itree_indC_spec. econs 12; eauto. gbase. eauto. }
-    { guclo sim_itree_indC_spec. econs 13; eauto. gbase. eauto. }
+    { guclo sim_itree_indC_spec. econs 9; eauto. des. esplits; eauto. gbase. eauto. }
+    { guclo sim_itree_indC_spec. econs 10; eauto. gbase. eauto. }
+    { guclo sim_itree_indC_spec. econs 11; eauto.  gbase. eauto. }
   Qed.
 
   Lemma sim_itreeC_spec r g
@@ -677,23 +586,24 @@ Section SIM.
     { i. eapply gupaco8_mon; eauto. }
   Qed.
 
-  Lemma sim_itree_progress_flag R0 R1 RR r g w st_src st_tgt
-        (SIM: gpaco8 _sim_itree (cpn8 _sim_itree) g g R0 R1 RR false false w st_src st_tgt)
+  Lemma sim_itree_progress_flag R0 R1 RR w r g st_src0 st_tgt0
+        (SIM: gpaco8 _sim_itree (cpn8 _sim_itree) g g R0 R1 RR false false w st_src0 st_tgt0)
     :
-      gpaco8 _sim_itree (cpn8 _sim_itree) r g R0 R1 RR true true w st_src st_tgt.
+      gpaco8 _sim_itree (cpn8 _sim_itree) r g R0 R1 RR true true w st_src0 st_tgt0.
   Proof.
-    gstep. destruct st_src, st_tgt. econs; eauto.
+    gstep. destruct st_src0, st_tgt0. econs; eauto. 
   Qed.
 
   Lemma sim_itree_flag_mon
-        (sim_itree: forall (R_src R_tgt: Type) (RR: st_local -> st_local -> R_src -> R_tgt -> Prop), bool -> bool -> world -> st_local * itree Es R_src -> st_local * itree Es R_tgt -> Prop)
+        (sim_itree: forall (R_src R_tgt: Type)
+                           (RR: st_local -> st_local -> R_src -> R_tgt -> Prop), bool -> bool -> world -> st_local * itree Es R_src -> st_local * itree Es R_tgt -> Prop)
         R_src R_tgt (RR: st_local -> st_local -> R_src -> R_tgt -> Prop)
-        f_src0 f_tgt0 f_src1 f_tgt1 w st_src st_tgt
-        (SIM: @_sim_itree sim_itree _ _ RR f_src0 f_tgt0 w st_src st_tgt)
+        f_src0 f_tgt0 f_src1 f_tgt1 w st_src0 st_tgt0
+        (SIM: @_sim_itree sim_itree _ _ RR f_src0 f_tgt0 w st_src0 st_tgt0)
         (SRC: f_src0 = true -> f_src1 = true)
         (TGT: f_tgt0 = true -> f_tgt1 = true)
     :
-      @_sim_itree sim_itree _ _ RR f_src1 f_tgt1 w st_src st_tgt.
+      @_sim_itree sim_itree _ _ RR f_src1 f_tgt1 w st_src0 st_tgt0.
   Proof.
     revert f_src1 f_tgt1 SRC TGT.
     induction SIM using _sim_itree_ind2; i; clarify.
@@ -701,28 +611,27 @@ Section SIM.
     { econs 2; eauto. }
     { econs 3; eauto. }
     { econs 4; eauto. }
-    { econs 5; eauto. des. esplits; eauto. }
-    { econs 6; eauto. i. exploit K; eauto. i. des. eauto. }
-    { econs 7; eauto. }
-    { econs 8; eauto. }
-    { econs 9; eauto. }
-    { econs 10; eauto. i. exploit K; eauto. i. des. eauto. }
-    { econs 11; eauto. des. esplits; eauto. }
-    { econs 12; eauto. }
-    { econs 13; eauto. }
-    { exploit SRC0; auto. exploit TGT0; auto. i. clarify. econs 14; eauto. }
+    { econs 5; eauto. } 
+    { econs 6; eauto. des. esplits; eauto. }
+    { econs 7; eauto. i. exploit K; eauto. i. des. eauto. }
+    { econs 8; eauto. i. exploit K; eauto. i. des. eauto. }
+    { econs 9; eauto. des. esplits; eauto. }
+    { econs 10; eauto. }
+    { econs 11; eauto. } 
+    { exploit SRC0; auto. exploit TGT0; auto. i. clarify. econs; eauto. }
   Qed.
 
-  Definition sim_fsem: relation (option mname * Any.t -> itree Es Any.t) :=
+
+  Definition sim_fsem: relation (Any.t -> itree Es Any.t) :=
     (eq ==> (fun it_src it_tgt => forall w mrs_src mrs_tgt (SIMMRS: wf w (mrs_src, mrs_tgt)),
                  sim_itree false false w (mrs_src, it_src)
                            (mrs_tgt, it_tgt)))%signature
   .
 
-  Definition sim_fnsem: relation (string * (option mname * Any.t -> itree Es Any.t)) := RelProd eq sim_fsem.
+  Definition sim_fnsem: relation (string * (Any.t -> itree Es Any.t)) := RelProd eq sim_fsem.
 
-
-  Variant lflagC (r: forall (R_src R_tgt: Type) (RR: st_local -> st_local -> R_src -> R_tgt -> Prop), bool -> bool -> world -> st_local * itree Es R_src -> st_local * itree Es R_tgt -> Prop)
+  Variant lflagC (r: forall (R_src R_tgt: Type)
+    (RR: st_local -> st_local -> R_src -> R_tgt -> Prop), bool -> bool -> world -> st_local * itree Es R_src -> st_local * itree Es R_tgt -> Prop)
           {R_src R_tgt} (RR: st_local -> st_local -> R_src -> R_tgt -> Prop)
     : bool -> bool -> world -> st_local * itree Es R_src -> st_local * itree Es R_tgt -> Prop :=
   | lflagC_intro
@@ -736,15 +645,15 @@ Section SIM.
 
   Lemma lflagC_mon
         r1 r2
-        (LE: r1 <8= r2)
+        (LE: r1  <8= r2)
     :
-      @lflagC r1 <8= @lflagC r2
+      @lflagC r1  <8= @lflagC r2
   .
   Proof. ii. destruct PR; econs; et. Qed.
 
   Hint Resolve lflagC_mon: paco.
 
-  Lemma lflagC_spec: lflagC <9= gupaco8 (_sim_itree) (cpn8 _sim_itree).
+  Lemma lflagC_spec: lflagC  <9= gupaco8 (_sim_itree) (cpn8 _sim_itree).
   Proof.
     eapply wrespect8_uclo; eauto with paco.
     econs; eauto with paco. i. inv PR.
@@ -755,56 +664,53 @@ Section SIM.
       esplits; eauto. eapply rclo8_base. eauto. }
     { econs 3; eauto. i. eapply rclo8_base. eauto. }
     { econs 4; eauto. }
-    { econs 5; eauto. des. esplits; eauto. }
-    { econs 6; eauto. i. exploit K; eauto. i. des. esplits; eauto. }
-    { econs 7; eauto. }
-    { econs 8; eauto. }
-    { econs 9; eauto. }
-    { econs 10; eauto. i. exploit K; eauto. i. des. esplits; eauto. }
-    { econs 11; eauto. des. esplits; eauto. }
-    { econs 12; eauto. }
-    { econs 13; eauto. }
-    { exploit SRC0; auto. exploit TGT0; auto. i. clarify. econs 14; eauto.
+    { econs 5; eauto. }
+    { econs 6; eauto.  des. esplits; eauto. }
+    { econs 7; eauto. i. exploit K; eauto. i. des. esplits; eauto. }
+    { econs 8; eauto. i. exploit K; eauto. i. des. esplits; eauto. }
+    { econs 9; eauto. des. esplits; eauto. }
+    { econs 10; eauto. }
+    { econs 11; eauto. }
+    { exploit SRC0; auto. exploit TGT0; auto. i. clarify. econs 12; eauto.
       eapply rclo8_base; auto. }
   Qed.
 
-  Lemma sim_itree_flag_down R0 R1 RR r g w st_src st_tgt f_src f_tgt
-        (SIM: gpaco8 _sim_itree (cpn8 _sim_itree) r g R0 R1 RR false false w st_src st_tgt)
+  Lemma sim_itree_flag_down  R0 R1 RR r g w st_src0 st_tgt0 f_src f_tgt
+        (SIM: gpaco8 _sim_itree (cpn8 _sim_itree) r g R0 R1 RR false false w st_src0 st_tgt0)
     :
-      gpaco8 _sim_itree (cpn8 _sim_itree) r g R0 R1 RR f_src f_tgt w st_src st_tgt.
+      gpaco8 _sim_itree (cpn8 _sim_itree) r g R0 R1 RR f_src f_tgt w st_src0 st_tgt0.
   Proof.
     guclo lflagC_spec. econs; eauto.
   Qed.
 
-  Lemma sim_itree_bot_flag_up R0 R1 RR w st_src st_tgt f_src f_tgt
-        (SIM: paco8 _sim_itree bot8 R0 R1 RR true true w st_src st_tgt)
+  Lemma sim_itree_bot_flag_up  R0 R1 RR w st_src0 st_tgt0 f_src f_tgt
+        (SIM: paco8 _sim_itree bot8 R0 R1 RR true true w st_src0 st_tgt0)
     :
-      paco8 _sim_itree bot8 R0 R1 RR f_src f_tgt w st_src st_tgt.
+      paco8 _sim_itree bot8 R0 R1 RR f_src f_tgt w st_src0 st_tgt0.
   Proof.
     ginit. remember true in SIM at 1. remember true in SIM at 1.
-    clear Heqb Heqb0. revert w st_src st_tgt f_src f_tgt b b0 SIM.
-    gcofix CIH. i. revert f_src f_tgt.
+    clear Heqb Heqb0. revert w st_src0 st_tgt0 f_src f_tgt b b0 SIM.
+    gcofix CIH. 
+    i. revert f_src f_tgt.
 
     (* TODO: why induction using sim_itree_ind doesn't work? *)
-    pattern b, b0, w, st_src, st_tgt.
+    pattern b, b0, w, st_src0, st_tgt0.
     match goal with
-    | |- ?P b b0 w st_src st_tgt => set P
+    | |- ?P b b0 w st_src0 st_tgt0 => set P
     end.
-    revert b b0 w st_src st_tgt SIM.
+    revert b b0 w st_src0 st_tgt0 SIM.
     eapply (@sim_itree_ind R0 R1 RR P); subst P; ss; i; clarify.
     { guclo sim_itree_indC_spec. econs 1; eauto. }
     { gstep. econs 2; eauto. i. gbase. eapply CIH; eauto. }
     { gstep. econs 3; eauto. i. gbase. eapply CIH; eauto. }
     { guclo sim_itree_indC_spec. econs 4; eauto. }
-    { guclo sim_itree_indC_spec. econs 5; eauto. des. esplits; eauto. }
-    { guclo sim_itree_indC_spec. econs 6; eauto. i. hexploit K; eauto. i. des. esplits; eauto. }
-    { guclo sim_itree_indC_spec. econs 7; eauto. }
-    { guclo sim_itree_indC_spec. econs 8; eauto. }
-    { guclo sim_itree_indC_spec. econs 9; eauto. }
-    { guclo sim_itree_indC_spec. econs 10; eauto. i. hexploit K; eauto. i. des. esplits; eauto. }
-    { guclo sim_itree_indC_spec. econs 11; eauto. des. esplits; eauto. }
-    { guclo sim_itree_indC_spec. econs 12; eauto. }
-    { guclo sim_itree_indC_spec. econs 13; eauto. }
+    { guclo sim_itree_indC_spec. econs 5; eauto. } 
+    { guclo sim_itree_indC_spec. econs 6; eauto. des. esplits; eauto. }
+    { guclo sim_itree_indC_spec. econs 7; eauto. i. hexploit K; eauto. i. des. esplits; eauto. }
+    { guclo sim_itree_indC_spec. econs 8; eauto. i. hexploit K; eauto. i. des. esplits; eauto. }
+    { guclo sim_itree_indC_spec. econs 9; eauto. des. esplits; eauto. }
+    { guclo sim_itree_indC_spec. econs 10; eauto. } 
+    { guclo sim_itree_indC_spec. econs 11; eauto. } 
     { eapply sim_itree_flag_down. gfinal. right.
       eapply paco8_mon; eauto. ss.
     }
@@ -814,7 +720,6 @@ Section SIM.
     forall S_src S_tgt (SS: st_local -> st_local -> S_src -> S_tgt -> Prop), bool -> bool -> world -> st_local * itree Es S_src -> st_local * itree Es S_tgt -> Prop :=
   | lbindR_intro
       f_src f_tgt w0 w1
-
       R_src R_tgt RR
       (st_src0 st_tgt0: st_local)
       (i_src: itree Es R_src) (i_tgt: itree Es R_tgt)
@@ -829,11 +734,11 @@ Section SIM.
 
   Hint Constructors lbindR: core.
 
-  Lemma lbindR_mon
+  Lemma lbindR_mon 
         r1 r2 s1 s2
-        (LEr: r1 <8= r2) (LEs: s1 <8= s2)
+        (LEr: r1  <8= r2) (LEs: s1  <8= s2)
     :
-      lbindR r1 s1 <8= lbindR r2 s2
+      lbindR r1 s1  <8= lbindR r2 s2
   .
   Proof. ii. destruct PR; econs; et. Qed.
 
@@ -859,24 +764,24 @@ Section SIM.
     + rewrite ! bind_bind. econs; eauto. i.
       eapply rclo8_clo_base. econs; eauto.
     + rewrite ! bind_tau. econs; eauto.
-    + rewrite ! bind_bind. econs; eauto. des. esplits; eauto.
-    + rewrite ! bind_bind. econs; eauto. i. exploit K; eauto. i. des. esplits; eauto.
-    + rewrite ! bind_bind. econs; eauto.
-    + rewrite ! bind_bind. econs; eauto.
     + rewrite ! bind_tau. econs; eauto.
+    + rewrite ! bind_bind. econs; eauto. des. esplits; eauto.
+    + rewrite ! bind_bind. econs; eauto. i. exploit K; eauto. i. des. esplits; eauto.
     + rewrite ! bind_bind. econs; eauto. i. exploit K; eauto. i. des. esplits; eauto.
     + rewrite ! bind_bind. econs; eauto. des. esplits; eauto.
-    + rewrite ! bind_bind. econs; eauto.
-    + rewrite ! bind_bind. econs; eauto.
+    + rewrite ! bind_bind. econs; eauto. 
+    + rewrite ! bind_bind. econs; eauto. 
     + econs; eauto. eapply rclo8_clo_base. econs; eauto.
   Qed.
 
-  Lemma lbindC_spec: lbindC <9= gupaco8 (_sim_itree) (cpn8 (_sim_itree)).
+  Lemma lbindC_spec: lbindC  <9= gupaco8 (_sim_itree) (cpn8 (_sim_itree)).
   Proof.
     intros. eapply wrespect8_uclo; eauto with paco. eapply lbindC_wrespectful.
   Qed.
 
 End SIM.
+
+
 Hint Resolve sim_itree_mon: paco.
 Hint Resolve cpn8_wcompat: paco.
 
@@ -896,22 +801,18 @@ Proof.
     eapply sim_itree_flag_down. gbase. auto.
   }
   destruct s.
-  { rewrite <- ! bind_trigger. resub. dependent destruction p.
-    { guclo sim_itree_indC_spec. econs.
-      guclo sim_itree_indC_spec. econs.
-      eapply sim_itree_progress_flag. gbase. auto.
-    }
+  { rewrite <- ! bind_trigger. resub. dependent destruction s.
     { guclo sim_itree_indC_spec. econs.
       guclo sim_itree_indC_spec. econs.
       eapply sim_itree_progress_flag. gbase. auto.
     }
   }
   { rewrite <- ! bind_trigger. resub. dependent destruction e.
-    { guclo sim_itree_indC_spec. econs 10. i.
+    { guclo sim_itree_indC_spec. econs 7. i.
       guclo sim_itree_indC_spec. econs. eexists.
       eapply sim_itree_progress_flag. gbase. eauto.
     }
-    { guclo sim_itree_indC_spec. econs 6. i.
+    { guclo sim_itree_indC_spec. econs 8. i.
       guclo sim_itree_indC_spec. econs. eexists.
       eapply sim_itree_progress_flag. gbase. eauto.
     }
@@ -920,7 +821,6 @@ Proof.
     }
   }
 Qed.
-
 
 
 (*** desiderata: (1) state-aware simulation relation !!!! ***)
@@ -941,8 +841,7 @@ Section SIMMODSEM.
     le: world -> world -> Prop;
     le_PreOrder: PreOrder le;
     sim_fnsems: Forall2 (sim_fnsem wf le) ms_src.(ModSem.fnsems) ms_tgt.(ModSem.fnsems);
-    sim_mn: ms_src.(ModSem.mn) = ms_tgt.(ModSem.mn);
-    sim_initial: exists w_init, wf w_init (ms_src.(ModSem.initial_st), ms_tgt.(ModSem.initial_st));
+    sim_initial: exists w_init, wf w_init (ms_src.(ModSem.init_st), ms_tgt.(ModSem.init_st));
   }.
 
 End SIMMODSEM.
@@ -954,12 +853,10 @@ Proof.
   - instantiate (1:=fun (_ _: unit) => True). ss.
   - instantiate (1:=(fun (_: unit) '(src, tgt) => src = tgt)). (* fun p => fst p = snd p *)
     generalize (ModSem.fnsems ms).
-    induction l; ii; ss.
+    induction a; ii; ss.
     econs; eauto. econs; ss. ii; clarify.
     destruct w. exploit self_sim_itree; et.
   - ss.
-Unshelve.
-all: try (exact 0).
 Qed.
 
 End ModSemPair.
@@ -993,25 +890,25 @@ Section SIMMOD.
 
   Context {CONF: EMSConfig}.
 
-  Lemma ModL_add_fnsems md0 md1 sk
+  Lemma Mod_add_fnsems md0 md1 sk
     :
-      (ModSemL.fnsems (ModL.get_modsem (ModL.add md0 md1) sk)) =
-      (ModSemL.fnsems (ModL.get_modsem md0 sk)) ++ (ModSemL.fnsems (ModL.get_modsem md1 sk)).
+      (ModSem.fnsems (Mod.get_modsem (Mod.add md0 md1) sk)) =
+      ModSem.add_fnsems (Mod.get_modsem md0 sk) (Mod.get_modsem md1 sk).
   Proof.
     ss.
   Qed.
 
-  Lemma ModL_add_sk md0 md1
+  Lemma Mod_add_sk md0 md1
     :
-      ModL.sk (ModL.add md0 md1) = ModL.sk md0 ++ ModL.sk md1.
+      Mod.sk (Mod.add md0 md1) = Mod.sk md0 ++ Mod.sk md1.
   Proof.
     ss.
   Qed.
-
+(* 
   Lemma Mod_list_incl_sk (mds: list Mod.t) md
         (IN: In md mds)
     :
-      Sk.incl (Mod.sk md) (ModL.sk (Mod.add_list mds)).
+      Sk.incl (Mod.sk md) (Mod.sk (Mod.add_list mds)).
   Proof.
     rewrite Mod.add_list_sk. revert IN. induction mds; ss.
     i. des; clarify.
@@ -1021,15 +918,19 @@ Section SIMMOD.
 
   Lemma Mod_add_list_get_modsem (mds: list Mod.t) sk
     :
-      ModL.get_modsem (Mod.add_list mds) sk
+      Mod.get_modsem (Mod.add_list mds) sk
       =
-      fold_right ModSemL.add {| ModSemL.fnsems := []; ModSemL.initial_mrs := [] |}
-                 (List.map (fun (md: Mod.t) => ModL.get_modsem md sk) mds).
+      fold_right ModSem.add {| ModSem.fnsems := []; ModSem.initial_mrs := [] |}
+                 (List.map (fun (md: Mod.t) => Mod.get_modsem md sk) mds).
   Proof.
     induction mds; ss. f_equal. rewrite <- IHmds. ss.
-  Qed.
+  Qed. *)
 
 End SIMMOD.
+
+
+
+
 
 Require Import SimGlobal.
 Require Import Red IRed.
@@ -1047,368 +948,252 @@ Module TAC.
 End TAC.
 Import TAC.
 
+Section SEMPAIR.
+  Variable ms_src: ModSem.t.
+  Variable ms_tgt: ModSem.t.
+  (* Variable ctx: ModSem.t.
+  Definition ms_src := ModSem.add ctx ms_src'.
+  Definition ms_tgt := ModSem.add ctx ms_tgt'. *)
+  (* Variable mn: mname. *)
+  Variable world: Type.
+  Variable wf: world -> Any.t * Any.t -> Prop.
+  Variable le: world -> world -> Prop.
+  Hypothesis le_PreOrder: PreOrder le.
+  
+  Hypothesis fnsems_find_iff:
+    forall fn,
+      (<<NONE: alist_find fn ms_src.(ModSem.fnsems) = None>>) \/
+      (exists (f: _ -> itree _ _) (ctx ms_src' ms_tgt': ModSem.t),
+          (<<CTX: alist_find fn ctx.(ModSem.fnsems) = Some f>>) /\
+          (<<SRC: ModSem.add ctx ms_src' = ms_src>>) /\
+          (<<TGT: ModSem.add ctx ms_tgt' = ms_tgt>>)) \/
+      (exists (f_src f_tgt: _ -> itree _ _),
+          (<<SRC: alist_find fn ms_src.(ModSem.fnsems) = Some f_src>>) /\
+          (<<TGT: alist_find fn ms_tgt.(ModSem.fnsems) = Some f_tgt>>) /\
+          (<<SIM: sim_fsem wf le f_src f_tgt>>)).
+          
+  Variant g_lift_rel
+          (w0: world) st_src0 st_tgt0: Prop :=
+  | g_lift_rel_intro
+      w1
+      (LE: le w0 w1)
+      (MN: wf w1 (st_src0, st_tgt0))
+      
+      (* (NMN: forall mn' (NIN: mn <> mn'), st_local mn' = st_local mn') *)
+  .
+  Variant my_r0:
+    forall R0 R1 (RR: R0 -> R1 -> Prop), bool -> bool -> (itree eventE R0) -> (itree eventE R1) -> Prop :=
+  | my_r0_intro
+      w0
+      (itr_src itr_tgt: itree Es Any.t)
+      st_src0 st_tgt0 o_src o_tgt
+      (SIM: sim_itree wf le o_src o_tgt w0 (st_src0, itr_src) (st_tgt0, itr_tgt))
+      (* (STATE: forall mn' (MN: mn <> mn'), st_local mn' = st_local mn') *)
+    :
+      my_r0 (fun '(st_src, ret_src) '(st_tgt, ret_tgt) =>
+                g_lift_rel w0 st_src st_tgt /\ ret_src = ret_tgt)
+            o_src o_tgt
+            (interp_Es (ModSem.prog ms_src) (itr_src) st_src0)
+            (interp_Es (ModSem.prog ms_tgt) (itr_tgt) st_tgt0)
+  .
 
-Section ADEQUACY.
-  Section SEMPAIR.
-    Variable ms_src: ModSemL.t.
-    Variable ms_tgt: ModSemL.t.
-
-    Variable mn: mname.
-    Variable world: Type.
-    Variable wf: world -> Any.t * Any.t -> Prop.
-    Variable le: world -> world -> Prop.
-
-    Hypothesis le_PreOrder: PreOrder le.
-
-    Hypothesis fnsems_find_iff:
-      forall fn,
-        (<<NONE: alist_find fn ms_src.(ModSemL.fnsems) = None>>) \/
-        (exists mn' (f: _ -> itree _ _),
-            (<<MN: mn <> mn'>>) /\
-            (<<SRC: alist_find fn ms_src.(ModSemL.fnsems) = Some (transl_all mn' (T:=Any.t) ∘ f)>>) /\
-            (<<TGT: alist_find fn ms_tgt.(ModSemL.fnsems) = Some (transl_all mn' (T:=Any.t) ∘ f)>>)) \/
-        (exists (f_src f_tgt: _ -> itree _ _),
-            (<<SRC: alist_find fn ms_src.(ModSemL.fnsems) = Some (transl_all mn (T:=Any.t) ∘ f_src)>>) /\
-            (<<TGT: alist_find fn ms_tgt.(ModSemL.fnsems) = Some (transl_all mn (T:=Any.t) ∘ f_tgt)>>) /\
-            (<<SIM: sim_fsem wf le f_src f_tgt>>)).
-
-
-    Variant g_lift_rel
-            (w0: world) (st_src st_tgt: p_state): Prop :=
-    | g_lift_rel_intro
-        w1
-        (LE: le w0 w1)
-        (MN: wf w1 (st_src mn, st_tgt mn))
-        (NMN: forall mn' (NIN: mn <> mn'), st_src mn' = st_tgt mn')
-    .
-
-    Variant my_r0:
-      forall R0 R1 (RR: R0 -> R1 -> Prop), bool -> bool -> (itree eventE R0) -> (itree eventE R1) -> Prop :=
-    | my_r0_intro
-        w0
-        (itr_src itr_tgt: itree Es Any.t)
-        st_src st_tgt o_src o_tgt
-        (SIM: sim_itree wf le o_src o_tgt w0 (st_src mn, itr_src) (st_tgt mn, itr_tgt))
-        (STATE: forall mn' (MN: mn <> mn'), st_src mn' = st_tgt mn')
-      :
-        my_r0 (fun '(st_src, ret_src) '(st_tgt, ret_tgt) =>
-                 g_lift_rel w0 st_src st_tgt /\ ret_src = ret_tgt)
-              o_src o_tgt
-              (EventsL.interp_Es (ModSemL.prog ms_src) (transl_all mn itr_src) st_src)
-              (EventsL.interp_Es (ModSemL.prog ms_tgt) (transl_all mn itr_tgt) st_tgt)
-    .
-
-    Variant my_r1:
-      forall R0 R1 (RR: R0 -> R1 -> Prop), bool -> bool -> (itree eventE R0) -> (itree eventE R1) -> Prop :=
-    | my_r1_intro
-        mn' w0 st_src st_tgt
-        (MN: mn <> mn')
+  Variant my_r1:
+    forall R0 R1 (RR: R0 -> R1 -> Prop), bool -> bool -> (itree eventE R0) -> (itree eventE R1) -> Prop :=
+  | my_r1_intro
+        w0 st_src st_tgt fn ctx 
+        (* ms_src' ms_tgt' *)
+        (CTX: exists f, alist_find fn ctx.(ModSem.fnsems) = Some f)
+        (* (SRC: ModSem.add ctx ms_src' = ms_src)
+        (TGT: ModSem.add ctx ms_tgt' = ms_tgt) *)
         (SIM: g_lift_rel w0 st_src st_tgt)
         (itr: itree Es Any.t)
-      :
-        my_r1 (fun '(st_src, ret_src) '(st_tgt, ret_tgt) =>
-                 g_lift_rel w0 st_src st_tgt /\ ret_src = ret_tgt)
-              false false
-              (EventsL.interp_Es (ModSemL.prog ms_src) (transl_all mn' itr) st_src)
-              (EventsL.interp_Es (ModSemL.prog ms_tgt) (transl_all mn' itr) st_tgt)
-    .
+    :
+      my_r1 (fun '(st_src, ret_src) '(st_tgt, ret_tgt) =>
+                g_lift_rel w0 st_src st_tgt /\ ret_src = ret_tgt)
+            false false
+            (interp_Es (ModSem.prog ms_src) (itr) st_src)
+            (interp_Es (ModSem.prog ms_tgt) (itr) st_tgt)
+  .
 
-    Let my_r := my_r0 \7/ my_r1.
-    Let sim_lift: my_r <7= simg.
-    Proof.
-      ginit.
-      { i. eapply cpn7_wcompat; eauto with paco. }
-      gcofix CIH. i. destruct PR.
-      { destruct H.
-        unfold sim_itree in SIM.
-        remember (st_src mn, itr_src).
-        remember (st_tgt mn, itr_tgt).
-        remember w0 in SIM at 2.
-        revert st_src itr_src st_tgt itr_tgt Heqp Heqp0 Heqw STATE.
+  Let my_r := my_r0 \7/ my_r1.
 
-        (* TODO: why induction using sim_itree_ind doesn't work? *)
-        pattern o_src, o_tgt, w, p, p0.
-        match goal with
-        | |- ?P o_src o_tgt w p p0 => set P
-        end.
-        revert o_src o_tgt w p p0 SIM.
-        eapply (@sim_itree_ind world wf le Any.t Any.t (lift_rel wf le w0 (@eq Any.t)) P); subst P; ss; i; clarify.
 
-        - rr in RET. des. step. splits; auto. econs; et.
-        - hexploit (fnsems_find_iff fn). i. des.
-          { steps. rewrite NONE. unfold unwrapU, triggerUB. step. ss. }
-          { steps. rewrite SRC. rewrite TGT. unfold unwrapU. ired_both.
-            apply simg_progress_flag.
-            guclo bindC_spec. econs.
-            { gbase. eapply CIH. right. econs; ss. econs; et. refl. }
-            { i. ss. des. destruct vret_src, vret_tgt. des; clarify. inv SIM.
-              hexploit K; et. i. des. pclearbot.
-              steps. gbase. eapply CIH. left. econs; et.
-            }
+
+  Let sim_lift: my_r <7= simg.
+  Proof.
+    ginit.
+    { i. eapply cpn7_wcompat; eauto with paco. }
+    gcofix CIH. i. destruct PR.
+
+    { destruct H.
+
+      unfold sim_itree in SIM.
+      remember (st_src0, itr_src).
+      remember (st_tgt0, itr_tgt).
+      remember w0 in SIM at 2.
+      revert st_src0 itr_src st_tgt0 itr_tgt Heqp Heqp0 Heqw.
+      (* TODO: why induction using sim_itree_ind doesn't work? *)
+      pattern o_src, o_tgt, w, p, p0.
+      match goal with
+      | |- ?P o_src o_tgt w p p0 => set P
+      end.
+      revert o_src o_tgt w p p0 SIM.
+      eapply (@sim_itree_ind world wf le Any.t Any.t (lift_rel wf le w0 (@eq Any.t)) P); subst P; ss; i; clarify.
+      - rr in RET. des. step. splits; auto. econs; et.
+      - hexploit (fnsems_find_iff fn). i. des.
+        { step. rewrite interp_Es_bind.  steps. rewrite NONE. unfold unwrapU, triggerUB. grind. step. ss. }
+        { steps. rewrite <- SRC, <- TGT. s. unfold ModSem.add_fnsems.
+          rewrite ! alist_find_app_o. unfold ModSem.trans_l.
+          rewrite ! alist_find_map. rewrite ! CTX. grind.
+          rewrite SRC, TGT.
+
+          apply simg_progress_flag. guclo bindC_spec. econs.
+          { gbase. eapply CIH.
+          
+          right. econs; ss. { eexists. apply CTX. } econs; et. refl.
+
+          (* econs; ss. grind. unfold sim_fsem, "==>" in SIM. et.  *)
           }
-          { hexploit (SIM (Some mn, varg) (Some mn, varg)); et. i. des.
-            steps. rewrite SRC. rewrite TGT. unfold unwrapU. ired_both.
-            apply simg_progress_flag.
-            guclo bindC_spec. econs.
-            { gbase. eapply CIH. left. econs; ss. et. }
-            { i. ss. destruct vret_src, vret_tgt. des; clarify. inv SIM0.
-              hexploit K; et. i. des. pclearbot.
-              steps. gbase. eapply CIH. left. econs; et.
-            }
-          }
-        - step. i. subst. apply simg_progress_flag.
-          hexploit (K x_tgt). i. des. pclearbot.
-          steps. gbase. eapply CIH. left. econs; et.
-        - ired_both. steps.
-        - des. force. exists x. steps. eapply IH; eauto.
-        - steps. i. hexploit K. i. des. steps. eapply IH; eauto.
-        - steps. eapply IH; eauto.
-          { unfold update. des_ifs. }
-          { i. unfold update. des_ifs. et. }
-        - steps. eapply IH; eauto.
-        - steps.
-        - steps. i. hexploit K. i. des. steps. eapply IH; eauto.
-        - des. force. exists x. steps. eapply IH; eauto.
-        - steps. eapply IH; eauto.
-          { unfold update. des_ifs. }
-          { i. unfold update. des_ifs. et. }
-        - steps. eapply IH; eauto.
-        - eapply simg_progress_flag. gbase. eapply CIH.
-          left. econs; eauto.
-      }
-      { destruct H. ides itr.
-        { steps. }
-        { steps. eapply simg_progress_flag. gbase. eapply CIH. right. econs; et. }
-        rewrite <- ! bind_trigger. destruct e.
-        { resub. destruct c. hexploit (fnsems_find_iff fn). i. des.
-          { steps. rewrite NONE. unfold unwrapU, triggerUB. step. ss. }
-          { inv SIM. steps. rewrite SRC. rewrite TGT. unfold unwrapU. ired_both.
-            guclo bindC_spec. econs.
-            { eapply simg_progress_flag. gbase. eapply CIH.
-              right. econs; ss. econs; et. }
-            { i. ss. des. destruct vret_src, vret_tgt. des; clarify.
-              steps. eapply simg_progress_flag.
-              gbase. eapply CIH. right. econs; et. }
-          }
-          { inv SIM. hexploit (SIM0 (Some mn', args) (Some mn', args)); et. i. des.
-            steps. rewrite SRC. rewrite TGT. unfold unwrapU. ired_both.
-            guclo bindC_spec. econs.
-            { eapply simg_progress_flag. gbase. eapply CIH. left. econs; ss. et. }
-            { i. ss. destruct vret_src, vret_tgt. des; clarify.
-              steps. eapply simg_progress_flag. gbase. eapply CIH. right. econs; et.
-              inv SIM. econs.
-              { etrans; et. }
-              { et. }
-              { et. }
-            }
+          { i. ss. destruct vret_src, vret_tgt. des; clarify. inv SIM.
+            hexploit K; et. i. des. pclearbot.
+            gbase. eapply CIH. left. econs; et.
+          }          
+        }
+
+        { hexploit (SIM (varg) (varg)); et. i. des. ired_both. 
+          steps. grind. rewrite SRC. rewrite TGT. unfold unwrapU. ired_both.
+          apply simg_progress_flag.
+          guclo bindC_spec. econs.
+          { gbase. eapply CIH. left. econs; ss. grind. et. }
+          { i. ss. destruct vret_src, vret_tgt. des; clarify. inv SIM0.
+            hexploit K; et. i. des. pclearbot. ired_both.
+            steps. gbase. eapply CIH. left. econs; et.
           }
         }
-        destruct s.
-        { resub. destruct p.
-          { steps. eapply simg_progress_flag.
-            gbase. eapply CIH. right. econs; et.
-            inv SIM. econs; et.
-            { unfold update. des_ifs. }
-            { ii. unfold update. des_ifs. et. }
-          }
-          { steps. eapply simg_progress_flag.
-            gbase. eapply CIH. right.
-            replace (st_tgt mn') with (st_src mn'); et.
-            { econs; et. }
-            { inv SIM. et. }
-          }
-        }
-        { resub. destruct e.
-          { steps. force. exists x. steps. eapply simg_progress_flag.
-            gbase. eapply CIH; et. right. econs; et.
-          }
-          { steps. force. exists x. steps. eapply simg_progress_flag.
-            gbase. eapply CIH; et. right. econs; et.
-          }
-          { steps. subst. eapply simg_progress_flag.
-            gbase. eapply CIH; et. right. econs; et. }
-        }
-      }
-    Qed.
-
-    Context `{CONF: EMSConfig}.
-
-    Hypothesis INIT:
-      exists w, g_lift_rel w (ModSemL.initial_p_state ms_src) (ModSemL.initial_p_state ms_tgt).
-
-    Lemma adequacy_local_aux (P Q: Prop)
-          (WF: Q -> P)
-      :
-        (Beh.of_program (ModSemL.compile ms_tgt (Some P)))
-        <1=
-        (Beh.of_program (ModSemL.compile ms_src (Some Q))).
-    Proof.
-      eapply adequacy_global_itree; ss.
-      hexploit INIT. i. des. ginit.
-      { eapply cpn7_wcompat; eauto with paco. }
-      unfold ModSemL.initial_itr, assume.
-      hexploit (fnsems_find_iff "main"). i. des.
-      { steps. unshelve esplits; et. unfold ITree.map, unwrapU, triggerUB. steps.
-        rewrite NONE. steps. ss. }
-      { steps. unshelve esplits; et. unfold ITree.map, unwrapU. steps.
-        rewrite SRC. rewrite TGT.
-        steps. force. esplits; et. steps.
+      - step. i. subst. apply simg_progress_flag.
+        hexploit (K x_tgt). i. des. pclearbot.
+        steps. gbase. eapply CIH. left. econs; et.
+      - steps.
+      - steps. 
+      - des. force. exists x. steps. eapply IH; eauto. 
+      - steps. i. hexploit K. i. des. steps. eapply IH; eauto.
+      - steps. i. hexploit K. i. des. steps. eapply IH; eauto.
+      - des. force. exists x. steps. eapply IH; eauto.
+      - steps. destruct run. steps. eapply IH; eauto.
+      - steps. destruct run. steps. eapply IH; eauto.
+      - eapply simg_progress_flag. gbase. eapply CIH. left. econs; eauto.
+    }
+    { destruct H. ides itr.
+    { steps. }
+    { steps. eapply simg_progress_flag. gbase. eapply CIH. right. econs; et. }
+    rewrite <- ! bind_trigger. destruct e.
+    { resub. destruct c. hexploit (fnsems_find_iff fn0). i. des.
+      {  steps.  rewrite NONE. unfold unwrapU, triggerUB. step. ss. }
+      { 
+        (* admit. *)
+        inv SIM. steps. (* Why no tau? *)
+        rewrite <- SRC. rewrite <- TGT. s.
+        unfold ModSem.add_fnsems.
+        rewrite ! alist_find_app_o. unfold ModSem.trans_l, ModSem.trans_r.
+        rewrite ! alist_find_map. rewrite CTX0. s. 
+        rewrite SRC, TGT.
+        ired_both. eapply simg_progress_flag.
         guclo bindC_spec. econs.
-        { eapply simg_progress_flag. gfinal. right. eapply sim_lift. right. econs; et. }
-        { i. destruct vret_src, vret_tgt. des; clarify. steps. }
+        { gbase. eapply CIH. right. econs; et. econs; et.  }
+        { i. ss. destruct vret_src, vret_tgt;et. des; clarify.
+            steps. gbase. eapply CIH. right. econs; et. }
       }
-      { inv H. hexploit (SIM (None, initial_arg) (None, initial_arg)); et. i. des.
-        steps. force. esplits; et.
-        steps. unfold ITree.map, unwrapU. steps.
-        rewrite SRC. rewrite TGT. steps. guclo bindC_spec. econs.
-        { eapply simg_flag_down. gfinal. right. eapply sim_lift. left. econs; et. }
-        { i. destruct vret_src, vret_tgt. des; clarify. steps. }
-      }
-      Unshelve. all: try exact 0.
-    Qed.
-  End SEMPAIR.
-
-  Theorem adequacy_local_strong md_src md_tgt
-          (SIM: ModPair.sim md_src md_tgt)
-    :
-      <<CR: (refines_strong md_tgt md_src)>>
-  .
-  Proof.
-    ii. unfold ModL.compile, ModL.enclose in *.
-    destruct (classic (ModL.wf (ModL.add (Mod.add_list ctx) md_src))).
-    2:{ eapply ModSemL.compile_not_wf. ss. }
-    pose (sk_tgt := (ModL.sk (ModL.add (Mod.add_list ctx) md_tgt))).
-    pose (sk_src := (ModL.sk (ModL.add (Mod.add_list ctx) md_src))).
-    assert (SKEQ: sk_tgt = sk_src).
-    { unfold sk_src, sk_tgt. ss. f_equal.
-      inv SIM. auto. }
-    rr in H. unfold ModL.enclose in *. fold sk_src in H. des. inv WF.
-    rename SK into SKWF.
-    rename wf_fnsems into FNWF.
-    rename wf_initial_mrs into MNWF.
-    inv SIM. hexploit (sim_modsem (Sk.canon sk_tgt)).
-    { etrans; [|eapply Sk.sort_incl]. ss. ii. eapply in_or_app. auto. }
-    { ss. fold sk_src in SKWF. rewrite SKEQ. clear - SKWF.
-      unfold Sk.wf in *. ss. eapply Permutation.Permutation_NoDup; [|et].
-      eapply Permutation.Permutation_map. eapply Sk.SkSort.sort_permutation. }
-    i. inv H. des.
-    assert (WFTGT: ModL.wf (ModL.add (Mod.add_list ctx) md_tgt)).
-    { rr. unfold ModL.enclose. fold sk_src sk_tgt.
-      rewrite SKEQ in *. split; auto. econs.
-      { clear MNWF.
-        match goal with
-        | H: NoDup ?l0 |- NoDup ?l1 => replace l1 with l0
-        end; auto. ss.
-        rewrite ! List.map_app. f_equal. rewrite ! List.map_map.
-        eapply Forall2_eq. eapply Forall2_apply_Forall2; et.
-        i. destruct a, b. inv H. ss.
-      }
-      { clear FNWF.
-        match goal with
-        | H: NoDup ?l0 |- NoDup ?l1 => replace l1 with l0
-        end; auto. ss.
-        rewrite ! List.map_app. f_equal. ss.
-        rewrite sim_mn. auto.
-      }
-    }
-    eapply adequacy_local_aux in PR; et.
-    { ss. ii. fold sk_src sk_tgt. rewrite <- SKEQ. rewrite ! alist_find_app_o. des_ifs.
-      { eapply alist_find_some in Heq.
-        rewrite Mod.add_list_fnsems in Heq.
-        rewrite <- fold_right_app_flat_map in Heq. ss.
-        eapply in_flat_map in Heq. des.
-        eapply in_map_iff in Heq0. des. destruct x1. ss. clarify.
-        right. left. esplits; ss; et.
-        instantiate (1:=ModSem.mn (Mod.get_modsem md_src (Sk.sort sk_tgt))).
-        ii. eapply NoDup_app_disjoint.
-        { rewrite List.map_app in MNWF. eapply MNWF. }
-        { rewrite Mod.add_list_initial_mrs.
-          rewrite <- fold_right_app_flat_map. eapply in_map.
-          eapply in_flat_map. ss. esplits; et. }
-        { ss. rewrite <- SKEQ. rewrite H. auto. }
-      }
-      { rewrite ! alist_find_map_snd. uo. des_ifs_safe ltac:(auto).
-        eapply alist_find_some in Heq0. right. right.
-        eapply Forall2_In_l in sim_fnsems; et. des. inv sim_fnsems0.
-        destruct b. esplits; ss; et. erewrite alist_find_some_iff; et.
-        { rewrite sim_mn. ss; et. }
-        { inv WFTGT. inv H1. ss. rewrite List.map_app in wf_fnsems.
-          apply nodup_app_r in wf_fnsems.
-          rewrite List.map_map in wf_fnsems. ss. fold sk_tgt in wf_fnsems.
-          erewrite List.map_ext; et. i. destruct a. ss.
+      { inv SIM. hexploit (SIM0 args args); et. i. des.
+        steps. rewrite SRC. rewrite TGT. unfold unwrapU. ired_both.
+        eapply simg_progress_flag.
+        guclo bindC_spec. econs.
+        { gbase. eapply CIH. left. econs; ss. et. }
+        { i. ss. destruct vret_src, vret_tgt. des; clarify.
+          steps. gbase. eapply CIH. right. econs; et.
+          inv SIM. econs.
+          { etrans; et. }
+          { et. }
         }
-        { ss. inv H. ss. clarify. }
       }
     }
-    { exists w_init. econs.
-      { refl. }
-      { unfold ModSemL.initial_p_state.
-        erewrite ! alist_find_some_iff; et.
-        { clear FNWF.
-          match goal with
-          | H: NoDup ?l0 |- NoDup ?l1 => replace l1 with l0
-          end; auto. ss.
-          fold sk_src. fold sk_tgt. rewrite <- SKEQ.
-          rewrite ! List.map_app. f_equal. ss. f_equal. auto.
-        }
-        { ss. eapply in_or_app. right. ss. left. fold sk_tgt. f_equal. auto. }
-        { ss. eapply in_or_app. right. ss. left. fold sk_src. rewrite SKEQ. auto. }
-      }
-      { ii. ss. fold sk_src sk_tgt. rewrite SKEQ. unfold ModSemL.initial_p_state.
-        ss. rewrite ! alist_find_app_o. des_ifs_safe.
-        rewrite <- SKEQ. ss. rewrite ! eq_rel_dec_correct. des_ifs. }
+    destruct s.
+    { resub. destruct s.
+      steps. grind. steps. eapply simg_progress_flag.
+      gbase. eapply CIH. right.
+      inv SIM.
+        replace (st_tgt mn') with (st_src mn'); et.
+        { econs; et. }
+        { inv SIM. et. }
+      
     }
+    { resub. destruct e.
+      { steps. force. exists x. steps. eapply simg_progress_flag.
+        gbase. eapply CIH; et. right. econs; et.
+      }
+      { steps. force. exists x. steps. eapply simg_progress_flag.
+        gbase. eapply CIH; et. right. econs; et.
+      }
+      { steps. subst. eapply simg_progress_flag.
+        gbase. eapply CIH; et. right. econs; et. }
+    }
+  }
   Qed.
-
-  Context {CONF: EMSConfig}.
-
-  Theorem adequacy_local md_src md_tgt
-          (SIM: ModPair.sim md_src md_tgt)
+  (* Admitted. *)
+  Context `{CONF: EMSConfig}.
+  Hypothesis INIT:
+    exists w, g_lift_rel w (ModSem.init_st ms_src) (ModSem.init_st ms_tgt).
+  Lemma adequacy_local_aux (P Q: Prop)
+        (* (wf: world -> W -> Prop)  *)
+        (WF: Q -> P)
     :
-      <<CR: (refines md_tgt md_src)>>
-  .
-  Proof.
-    eapply ModSem.refines_strong_refines.
-    eapply adequacy_local_strong; et.
+      (Beh.of_program (ModSem.compile ms_tgt (Some P)))
+      <1=
+      (Beh.of_program (ModSem.compile ms_src (Some Q))).
+  Proof. 
+    eapply adequacy_global_itree; ss.
+    hexploit INIT. i. 
+    des. ginit.
+    { eapply cpn7_wcompat; eauto with paco. }
+    unfold ModSem.initial_itr, assume. generalize "main" as fn. i.
+    hexploit (fnsems_find_iff fn). i. des.
+    { steps. unshelve esplits; et. unfold ITree.map, unwrapU, triggerUB. steps.
+      rewrite NONE. steps. ss. }
+    (* { admit. } *)
+    { 
+      inv H. rewrite <- SRC, <- TGT in *.
+      hexploit (SIM (initial_arg) (initial_arg)) ; et; cycle 1. i. des.
+      steps. force. esplits; et.
+      steps. unfold ITree.map, unwrapU.
+      rewrite ! interp_Es_bind. rewrite ! bind_bind.
+       s. unfold ModSem.add_fnsems.
+      rewrite ! alist_find_app_o. unfold ModSem.trans_l.
+      rewrite ! alist_find_map. rewrite CTX.
+      steps. rewrite SRC, TGT.
+      guclo bindC_spec. econs.
+      { eapply simg_flag_down. gfinal. right. eapply sim_lift. econs; et. }
+      { i. destruct vret_src, vret_tgt. des; clarify. steps. }
+    }
+    { 
+      inv H. 
+      hexploit (SIM (initial_arg) (initial_arg)) ; et; cycle 1. i. des.
+      steps. force. esplits; et.
+      steps. unfold ITree.map, unwrapU.
+      rewrite ! interp_Es_bind. rewrite ! bind_bind.
+      rewrite SRC. rewrite TGT. steps. guclo bindC_spec. econs.
+      { eapply simg_flag_down. gfinal. right. eapply sim_lift. econs; et. }
+      { i. destruct vret_src, vret_tgt. des; clarify. steps. }
+    }
+    
+  (* Admitted. *)
   Qed.
+  Definition wf_lift wf :=
+    fun (w:world) => 
+    (fun '(src, tgt) =>
+      match (Any.split src), (Any.split tgt) with
+      | Some (l1, r1), Some (l2, r2) => l1 = l2 /\ wf w (r1, r2)
+      | _, _ => wf w (src, tgt)
+      end
+    ).
+End SEMPAIR.
 
-  Corollary adequacy_local_list_strong
-            mds_src mds_tgt
-            (FORALL: List.Forall2 ModPair.sim mds_src mds_tgt)
-    :
-      <<CR: refines_strong (Mod.add_list mds_tgt) (Mod.add_list mds_src)>>
-  .
-  Proof.
-    r. induction FORALL; ss.
-    { ii. auto. }
-    rewrite ! Mod.add_list_cons.
-    etrans.
-    { rewrite <- Mod.add_list_single. eapply refines_strong_proper_r.
-      rewrite ! Mod.add_list_single. eapply adequacy_local_strong; et. }
-    replace (Mod.lift x) with (Mod.add_list [x]); cycle 1.
-    { cbn. rewrite ModL.add_empty_r. refl. }
-    eapply refines_strong_proper_l; et.
-  Qed.
 
-  Theorem adequacy_local2 md_src md_tgt
-          (SIM: ModPair.sim md_src md_tgt)
-    :
-      <<CR: (refines2 [md_tgt] [md_src])>>
-  .
-  Proof.
-    eapply ModSem.refines_strong_refines.
-    eapply adequacy_local_list_strong. econs; ss.
-  Qed.
-
-  Corollary adequacy_local_list
-            mds_src mds_tgt
-            (FORALL: List.Forall2 ModPair.sim mds_src mds_tgt)
-    :
-      <<CR: refines (Mod.add_list mds_tgt) (Mod.add_list mds_src)>>
-  .
-  Proof.
-    eapply ModSem.refines_strong_refines.
-    eapply adequacy_local_list_strong; et.
-  Qed.
-
-End ADEQUACY.
