ems/ModSemFacts.v
@@ -1,0 +1,882 @@
+Require Import Coqlib.
+Require Export sflib.
+Require Export ITreelib.
+Require Import STS Behavior.
+Require Import ModSem.
+Require Import SimGlobal.
+Require Import Skeleton.
+Require Import STS Behavior.
+Require Import Any.
+Require Import Red IRed.
+Require Import SimModSem.
+
+Require Import Behavior.
+Require Import Relation_Definitions.
+
+(*** TODO: export these in Coqlib or Universe ***)
+Require Import Relation_Operators.
+Require Import RelationPairs.
+From ITree Require Import
+     Events.MapDefault
+     TranslateFacts.
+From ExtLib Require Import
+     Core.RelDec
+     Structures.Maps
+     Data.Map.FMapAList.
+Require Import Any.
+
+
+Set Implicit Arguments.
+
+
+Module ModSemFacts.
+Import ModSem.
+Section COMM.
+
+  Inductive comm_emb : IFun Es Es -> IFun Es Es -> Prop := 
+    |comm_emb_1 : comm_emb emb_l emb_r
+    |comm_emb_2 : comm_emb emb_r emb_l
+  .
+
+  Inductive comm_ems : itree Es Any.t -> itree Es Any.t -> Prop := 
+    | comm_ems_intro emb_l emb_r it (EMB: comm_emb emb_l emb_r) :
+        comm_ems (translate emb_l it) (translate emb_r it).    
+
+  Definition comm_st (stp: Any.t * Any.t) : Prop :=
+    exists a b, fst stp = Any.pair a b /\ 
+    snd stp = Any.pair b a.
+
+  Lemma add_comm_aux
+        itl itr stl str (w: unit)
+        (COMM: comm_ems itl itr)
+        (STATE: comm_st (stl, str))
+
+  :
+      sim_itree (fun _ => comm_st) top2 false false w (stl, itl) (str, itr).
+  Proof.   
+    destruct COMM, STATE. des. ss.
+    (* unfold assoc_st. *)
+    ginit. 
+    generalize it as itr. 
+    clarify.
+    generalize x as a0.
+    generalize b as b0.
+    gcofix CIH. i.
+    rewrite (itree_eta_ itr).
+    destruct (observe itr).
+    - erewrite ! (bisimulation_is_eq _ _ (translate_ret _ _)).
+      gstep. apply sim_itree_ret.
+      unfold lift_rel. 
+      eexists; et. splits; et.
+      unfold comm_st. exists a0, b0; et.
+    - erewrite ! (bisimulation_is_eq _ _ (translate_tau _ _)).
+      gstep. 
+      apply sim_itree_tau_src. apply sim_itree_tau_tgt. 
+      eapply sim_itree_progress; et.
+      gfinal. left. eapply CIH; et.
+    - erewrite ! (bisimulation_is_eq _ _ (translate_vis _ _ _ _)).
+      rewrite <- ! bind_trigger.
+      destruct e as [c|[s|e]].
+      + (* callE *)
+        gstep. destruct c, EMB. 
+        (* SIMPLIFY BELOW *)
+        * apply sim_itree_call; clarify.
+          -- exists a0, b0; et.
+          -- i. unfold comm_st in WF. des. ss. clarify.
+           gfinal. left. eapply CIH.
+        * apply sim_itree_call; clarify.
+          -- eexists a0, b0; et.
+          -- i. unfold comm_st in WF. des. ss. clarify.
+             gfinal. left. eapply CIH.
+
+      + (* sE *)
+        gstep. destruct s, EMB.
+        * apply sim_itree_supdate_src. apply sim_itree_supdate_tgt.
+          eapply sim_itree_progress; et.
+          unfold run_l, run_r. rewrite ! Any.pair_split.
+          gfinal. left. destruct (run a0). eapply CIH.
+        * apply sim_itree_supdate_src. apply sim_itree_supdate_tgt.
+          eapply sim_itree_progress; et.
+          unfold run_l, run_r. rewrite ! Any.pair_split.
+          gfinal. left. destruct (run b0). eapply CIH.  
+      + (* eventE *)
+        gstep. destruct e, EMB.
+        (* Choose *)
+        * apply sim_itree_choose_tgt. i. apply sim_itree_choose_src. exists x0.
+          eapply sim_itree_progress; et.
+          gfinal. left. eapply CIH.
+        * apply sim_itree_choose_tgt. i. apply sim_itree_choose_src. exists x0.
+          eapply sim_itree_progress; et.
+          gfinal. left. eapply CIH.
+        (* Take *)
+        * apply sim_itree_take_src. i. apply sim_itree_take_tgt. exists x0.
+          eapply sim_itree_progress; et.
+          gfinal. left. eapply CIH. 
+        * apply sim_itree_take_src. i. apply sim_itree_take_tgt. exists x0.
+          eapply sim_itree_progress; et.
+          gfinal. left. eapply CIH. 
+        (* Syscall *)
+        * apply sim_itree_syscall. i.
+          eapply sim_itree_flag_down.
+          gfinal. left. eapply CIH. 
+        * apply sim_itree_syscall. i.
+          eapply sim_itree_flag_down.
+          gfinal. left. eapply CIH.
+  Qed. 
+
+
+  (* Move to somewhere else *)
+  Lemma fst_trans_l : forall x, fst (trans_l x) = fst x.
+  Proof. i. destruct x. ss. Qed.
+
+  Lemma fst_trans_r : forall x, fst (trans_r x) = fst x.
+  Proof. i. destruct x. ss. Qed.
+
+  Context {CONF: EMSConfig}.
+
+  Theorem add_comm
+    ms0 ms1
+    (P0 P1: Prop) (IMPL: P1 -> P0)
+    (WF: wf (add ms1 ms0))
+  :
+  <<COMM: Beh.of_program (compile (add ms0 ms1) (Some P0)) <1= Beh.of_program (compile (add ms1 ms0) (Some P1))>>
+  .
+  Proof.
+    destruct (classic (P1)); cycle 1.
+    { ii. eapply initial_itr_not_wf;et. }
+    replace P0 with P1.
+    2: { eapply prop_ext. split; auto. }
+    unfold compile. red. eapply adequacy_local_aux; et.
+    - i. s.
+      unfold add_fnsems. rewrite ! alist_find_app_o.
+      destruct (alist_find fn (fnsems ms1)) eqn:MS1; destruct (alist_find fn (fnsems ms0)) eqn: MS0.
+      + right. right. unfold trans_l.
+        exists (fun args => translate emb_l (i args)).
+        exists (fun args => translate emb_r (i args)).
+        rewrite ! alist_find_map.
+        esplits; et.
+        * rewrite MS1. et.
+        * inv WF. ss. unfold add_fnsems in wf_fnsems0. 
+          rewrite ! List.map_app in *. rewrite ! List.map_map in *.
+          apply NoDup_app_disjoint with (a:=fn) in wf_fnsems0.
+          -- clarify.
+          -- replace fn with (fst (fn, i)); et.
+             replace (fun x : string * (Any.t -> itree Es Any.t) => fst (trans_l x)) with (fun x : string * (Any.t -> itree Es Any.t) => fst x).
+             2: { extensionality x. rewrite fst_trans_l. et. }
+             apply in_map. apply alist_find_some in MS1. et. 
+          -- replace fn with (fst (fn, i0)); et.
+             replace (fun x : string * (Any.t -> itree Es Any.t) => fst (trans_r x)) with (fun x : string * (Any.t -> itree Es Any.t) => fst x).
+             2: { extensionality x. rewrite fst_trans_r. et. }
+             apply in_map. apply alist_find_some in MS0. et.
+        * instantiate (1:= top2). instantiate (1:= unit). instantiate (1:=(fun _ => comm_st)).
+          unfold sim_fsem, "==>". i. eapply add_comm_aux; et.
+          rewrite H0. econs. econs.
+      + right. right. unfold trans_l.
+        exists (fun args => translate emb_l (i args)).
+        exists (fun args => translate emb_r (i args)).          
+        rewrite ! alist_find_map.
+        esplits; et.
+        * rewrite MS1. et.
+        * rewrite MS0. s. unfold trans_r. rewrite alist_find_map.
+          unfold o_map. rewrite MS1. et.
+        * unfold sim_fsem, "==>". i. eapply add_comm_aux; et.
+          rewrite H0. econs. econs.
+
+      + right. right. unfold trans_l.
+        exists (fun args => translate emb_r (i args)).
+        exists (fun args => translate emb_l (i args)).          
+        rewrite ! alist_find_map.
+        esplits; et.        
+        * rewrite MS1. s. unfold trans_r. rewrite alist_find_map.
+          unfold o_map. rewrite MS0. et.
+        * rewrite MS0. et.
+        * unfold sim_fsem, "==>". i. eapply add_comm_aux; et.
+          rewrite H0. econs. econs.
+      + left. unfold trans_l, trans_r.
+        rewrite ! alist_find_map. rewrite MS1, MS0. et.
+    - exists tt. econs; et; clarify.
+      unfold comm_st. ss. exists (init_st ms1), (init_st ms0). et.
+Qed.
+
+End COMM.
+Section ASSOC.
+
+Inductive assoc_emb : IFun Es Es -> IFun Es Es -> Prop := 
+  |assoc_emb_1 : assoc_emb emb_l (emb_l >>> emb_l)
+  |assoc_emb_2 : assoc_emb (emb_l >>> emb_r ) (emb_r >>> emb_l)
+  |assoc_emb_3 : assoc_emb (emb_r >>> emb_r) emb_r
+.
+
+Inductive assoc_ems : itree Es Any.t -> itree Es Any.t -> Prop := 
+  | assoc_ems_intro emb_l emb_r it (EMB: assoc_emb emb_l emb_r) :
+      assoc_ems (translate emb_l it) (translate emb_r it).
+     
+Definition assoc_st (stp: Any.t * Any.t) : Prop :=
+  exists a b c, fst stp = Any.pair a (Any.pair b c) /\ 
+  snd stp = Any.pair (Any.pair a b) c
+.
+
+Definition assoc_rev_st (stp: Any.t * Any.t) : Prop :=
+  exists a b c, fst stp = Any.pair (Any.pair a b) c /\ 
+  snd stp = Any.pair a (Any.pair b c)
+.
+
+Lemma add_assoc_aux
+        itl itr stl str (w: unit)
+        (ASSOC: assoc_ems itl itr)
+        (STATE: assoc_st (stl, str))
+
+  :
+      sim_itree (fun _ => assoc_st) top2 false false w (stl, itl) (str, itr).
+Proof.
+  destruct ASSOC, STATE. des. ss.
+  (* unfold assoc_st. *)
+  ginit. 
+  generalize it as itr. 
+  clarify.
+  generalize x as a0.
+  generalize b as b0.
+  generalize c as c0.
+  gcofix CIH. i.
+  rewrite (itree_eta_ itr).
+  destruct (observe itr).
+  - erewrite ! (bisimulation_is_eq _ _ (translate_ret _ _)).
+    gstep. apply sim_itree_ret.
+    unfold lift_rel. 
+    exists tt. splits; et.
+    unfold assoc_st. exists a0, b0, c0; et.
+  - erewrite ! (bisimulation_is_eq _ _ (translate_tau _ _)).
+    gstep. 
+    apply sim_itree_tau_src. apply sim_itree_tau_tgt. 
+    eapply sim_itree_progress; et.
+    gfinal. left. eapply CIH; et.
+  - erewrite ! (bisimulation_is_eq _ _ (translate_vis _ _ _ _)).
+    rewrite <- ! bind_trigger.
+    destruct e as [c'|[s|e]].
+    + (* callE *)
+      gstep. destruct c', EMB. 
+      (* SIMPLIFY BELOW *)
+      * apply sim_itree_call; clarify.
+        -- exists a0, b0, c0; et.
+        -- i. destruct WF, H, H, H. ss. clarify.
+         gfinal. left. eapply CIH.
+      * apply sim_itree_call; clarify.
+        -- eexists a0, b0, c0; et.
+        -- i. unfold assoc_st in WF. des. ss. clarify.
+           gfinal. left. eapply CIH.
+      * apply sim_itree_call; clarify.
+        -- eexists a0, b0, c0; et.
+        -- i. unfold assoc_st in WF. des. ss. clarify.
+           gfinal. left. eapply CIH. 
+    + (* sE *)
+      gstep. destruct s, EMB.
+      * apply sim_itree_supdate_src. apply sim_itree_supdate_tgt.
+        eapply sim_itree_progress; et.
+        unfold run_l, run_r. rewrite ! Any.pair_split.
+        gfinal. left. destruct (run a0). eapply CIH.
+      * apply sim_itree_supdate_src. apply sim_itree_supdate_tgt.
+        eapply sim_itree_progress; et.
+        unfold run_l, run_r. rewrite ! Any.pair_split.
+        gfinal. left. destruct (run b0). eapply CIH.
+      * apply sim_itree_supdate_src. apply sim_itree_supdate_tgt.
+        eapply sim_itree_progress; et.
+        unfold run_l, run_r. rewrite ! Any.pair_split.
+        gfinal. left. destruct (run c0). eapply CIH.        
+    + (* eventE *)
+      gstep. destruct e, EMB.
+      (* Choose *)
+      * apply sim_itree_choose_tgt. i. apply sim_itree_choose_src. exists x0.
+        eapply sim_itree_progress; et.
+        gfinal. left. eapply CIH.
+      * apply sim_itree_choose_tgt. i. apply sim_itree_choose_src. exists x0.
+        eapply sim_itree_progress; et.
+        gfinal. left. eapply CIH.
+      * apply sim_itree_choose_tgt. i. apply sim_itree_choose_src. exists x0.
+        eapply sim_itree_progress; et.
+        gfinal. left. eapply CIH.
+      (* Take *)
+      * apply sim_itree_take_src. i. apply sim_itree_take_tgt. exists x0.
+        eapply sim_itree_progress; et.
+        gfinal. left. eapply CIH. 
+      * apply sim_itree_take_src. i. apply sim_itree_take_tgt. exists x0.
+        eapply sim_itree_progress; et.
+        gfinal. left. eapply CIH. 
+      * apply sim_itree_take_src. i. apply sim_itree_take_tgt. exists x0.
+        eapply sim_itree_progress; et.
+        gfinal. left. eapply CIH.
+      (* Syscall *)
+      * apply sim_itree_syscall. i.
+        eapply sim_itree_flag_down.
+        gfinal. left. eapply CIH. 
+      * apply sim_itree_syscall. i.
+        eapply sim_itree_flag_down.
+        gfinal. left. eapply CIH.
+      * apply sim_itree_syscall. i.
+        eapply sim_itree_flag_down.
+        gfinal. left. eapply CIH.
+Qed. 
+
+Lemma add_assoc_rev_aux
+        itl itr stl str (w: unit)
+        (ASSOC: assoc_ems itr itl)
+        (STATE: assoc_rev_st (stl, str))
+
+  :
+      sim_itree (fun _ => assoc_rev_st) top2 false false w (stl, itl) (str, itr)
+.
+Proof.
+destruct ASSOC, STATE. des. ss.
+(* unfold assoc_st. *)
+ginit. 
+generalize it as itr. 
+clarify.
+generalize x as a0.
+generalize b as b0.
+generalize c as c0.
+gcofix CIH. i.
+rewrite (itree_eta_ itr).
+destruct (observe itr).
+- erewrite ! (bisimulation_is_eq _ _ (translate_ret _ _)).
+  gstep. apply sim_itree_ret.
+  unfold lift_rel. 
+  exists tt. splits; et.
+  unfold assoc_st. exists a0, b0, c0; et.
+- erewrite ! (bisimulation_is_eq _ _ (translate_tau _ _)).
+  gstep. 
+  apply sim_itree_tau_src. apply sim_itree_tau_tgt. 
+  eapply sim_itree_progress; et.
+  gfinal. left. eapply CIH; et.
+- erewrite ! (bisimulation_is_eq _ _ (translate_vis _ _ _ _)).
+  rewrite <- ! bind_trigger.
+  destruct e as [c'|[s|e]].
+  + (* callE *)
+    gstep. destruct c', EMB. 
+    (* SIMPLIFY BELOW *)
+    * apply sim_itree_call; clarify.
+      -- exists a0, b0, c0; et.
+      -- i. destruct WF, H, H, H. ss. clarify.
+       gfinal. left. eapply CIH.
+    * apply sim_itree_call; clarify.
+      -- eexists a0, b0, c0; et.
+      -- i. unfold assoc_rev_st in WF. des. ss. clarify.
+         gfinal. left. eapply CIH.
+    * apply sim_itree_call; clarify.
+      -- eexists a0, b0, c0; et.
+      -- i. unfold assoc_rev_st in WF. des. ss. clarify.
+         gfinal. left. eapply CIH. 
+  + (* sE *)
+    gstep. destruct s, EMB.
+    * apply sim_itree_supdate_src. apply sim_itree_supdate_tgt.
+      eapply sim_itree_progress; et.
+      unfold run_l, run_r. rewrite ! Any.pair_split.
+      gfinal. left. destruct (run a0). eapply CIH.
+    * apply sim_itree_supdate_src. apply sim_itree_supdate_tgt.
+      eapply sim_itree_progress; et.
+      unfold run_l, run_r. rewrite ! Any.pair_split.
+      gfinal. left. destruct (run b0). eapply CIH.
+    * apply sim_itree_supdate_src. apply sim_itree_supdate_tgt.
+      eapply sim_itree_progress; et.
+      unfold run_l, run_r. rewrite ! Any.pair_split.
+      gfinal. left. destruct (run c0). eapply CIH.        
+  + (* eventE *)
+    gstep. destruct e, EMB.
+    (* Choose *)
+    * apply sim_itree_choose_tgt. i. apply sim_itree_choose_src. exists x0.
+      eapply sim_itree_progress; et.
+      gfinal. left. eapply CIH.
+    * apply sim_itree_choose_tgt. i. apply sim_itree_choose_src. exists x0.
+      eapply sim_itree_progress; et.
+      gfinal. left. eapply CIH.
+    * apply sim_itree_choose_tgt. i. apply sim_itree_choose_src. exists x0.
+      eapply sim_itree_progress; et.
+      gfinal. left. eapply CIH.
+    (* Take *)
+    * apply sim_itree_take_src. i. apply sim_itree_take_tgt. exists x0.
+      eapply sim_itree_progress; et.
+      gfinal. left. eapply CIH. 
+    * apply sim_itree_take_src. i. apply sim_itree_take_tgt. exists x0.
+      eapply sim_itree_progress; et.
+      gfinal. left. eapply CIH. 
+    * apply sim_itree_take_src. i. apply sim_itree_take_tgt. exists x0.
+      eapply sim_itree_progress; et.
+      gfinal. left. eapply CIH.
+    (* Syscall *)
+    * apply sim_itree_syscall. i.
+      eapply sim_itree_flag_down.
+      gfinal. left. eapply CIH. 
+    * apply sim_itree_syscall. i.
+      eapply sim_itree_flag_down.
+      gfinal. left. eapply CIH.
+    * apply sim_itree_syscall. i.
+      eapply sim_itree_flag_down.
+      gfinal. left. eapply CIH.
+Qed. 
+
+Context {CONF: EMSConfig}.
+
+
+Theorem add_assoc
+        ms0 ms1 ms2
+        (P0 P1: Prop) (IMPL: P1 -> P0)
+        (WF: wf (add ms0 (add ms1 ms2)))
+  :
+    <<COMM: Beh.of_program (compile (add (add ms0 ms1) ms2) (Some P0)) <1=
+            Beh.of_program (compile (add ms0 (add ms1 ms2)) (Some P1))>>
+.
+Proof. 
+  destruct (classic (P1)); cycle 1.
+  { ii. eapply initial_itr_not_wf;et. }
+  replace P0 with P1.
+  2: { eapply prop_ext. split; auto. }
+  unfold compile. red. 
+  eapply adequacy_local_aux; et.
+  2: { exists tt. instantiate (1:= top2). instantiate (1:=(fun _ => assoc_st)).  econs; et; clarify. 
+       unfold assoc_st. ss. exists (init_st ms0), (init_st ms1), (init_st ms2). splits; et. }
+  i. s.
+  unfold add_fnsems, trans_l, trans_r. s. unfold add_fnsems, trans_l, trans_r. 
+  rewrite ! alist_find_app_o. rewrite ! alist_find_map. 
+  rewrite ! alist_find_app_o. rewrite ! alist_find_map. 
+  destruct (alist_find fn (fnsems ms0)) eqn: MS0; destruct (alist_find fn (fnsems ms1)) eqn:MS1; destruct (alist_find fn (fnsems ms2)) eqn: MS2.
+  - inv WF. ss. unfold add_fnsems in wf_fnsems0. ss. unfold add_fnsems in wf_fnsems0.
+    rewrite ! List.map_app in *. rewrite ! List.map_map in *.
+    apply NoDup_app_disjoint with (a:=fn) in wf_fnsems0; ss.
+    + replace fn with (fst (fn, i)); et.
+      replace (fun x : string * (Any.t -> itree Es Any.t) => fst (trans_l x)) with (fun x : string * (Any.t -> itree Es Any.t) => fst x).
+      2: { extensionality x. rewrite fst_trans_l. et. }
+      apply in_map. apply alist_find_some in MS0. et.
+    + replace fn with (fst (fn, i0)); et.
+      replace (fun x : string * (Any.t -> itree Es Any.t) => fst (trans_r (trans_l x))) with (fun x : string * (Any.t -> itree Es Any.t) => fst x).
+      2: { extensionality x. rewrite fst_trans_r. rewrite fst_trans_l. et. }
+      apply in_app_iff. left. 
+      apply in_map. apply alist_find_some in MS1. et.
+  - inv WF. ss. unfold add_fnsems in wf_fnsems0. ss. unfold add_fnsems in wf_fnsems0.
+    rewrite ! List.map_app in *. rewrite ! List.map_map in *.
+    apply NoDup_app_disjoint with (a:=fn) in wf_fnsems0; ss.
+    + replace fn with (fst (fn, i)); et.
+      replace (List.map (fun x : string * (Any.t -> itree Es Any.t) => fst (trans_l x))) with (List.map (fun x : string * (Any.t -> itree Es Any.t) => fst x)).
+      2: { f_equal. extensionality x. rewrite fst_trans_l. et. }
+      apply in_map. apply alist_find_some in MS0. et.
+    + replace fn with (fst (fn, i0)); et.
+      replace (fun x : string * (Any.t -> itree Es Any.t) => fst (trans_r (trans_l x))) with (fun x : string * (Any.t -> itree Es Any.t) => fst x).
+      2: { extensionality x. rewrite fst_trans_r. rewrite fst_trans_l. et. }
+      apply in_app_iff. left. apply in_map.
+      apply alist_find_some in MS1. et.
+  - inv WF. ss. unfold add_fnsems in wf_fnsems0. ss. unfold add_fnsems in wf_fnsems0.
+    rewrite ! List.map_app in *. rewrite ! List.map_map in *.
+    apply NoDup_app_disjoint with (a:=fn) in wf_fnsems0; ss.
+    + replace fn with (fst (fn, i)); et.
+      replace (List.map (fun x : string * (Any.t -> itree Es Any.t) => fst (trans_l x))) with (List.map (fun x : string * (Any.t -> itree Es Any.t) => fst x)).
+      2: { f_equal. extensionality x. rewrite fst_trans_l. et. }
+      apply in_map. apply alist_find_some in MS0. et.
+    + replace fn with (fst (fn, i0)); et.
+      replace (fun x : string * (Any.t -> itree Es Any.t) => fst (trans_r (trans_r x))) with (fun x : string * (Any.t -> itree Es Any.t) => fst x).
+      2: { extensionality x. rewrite fst_trans_r. rewrite fst_trans_r. et. }
+      apply in_app_iff. right. apply in_map.
+      apply alist_find_some in MS2. et.
+  - right. right. esplits; et; s; et.
+    unfold sim_fsem, "==>". i. eapply add_assoc_aux; et.
+    rewrite H0. 
+    erewrite <- (@bisimulation_is_eq _ _ _ _ (@translate_cmpE _ _ _ _ _ _ _)).
+    econs. econs.
+  - inv WF. ss. unfold add_fnsems in wf_fnsems0. ss. unfold add_fnsems in wf_fnsems0.
+    rewrite ! List.map_app in *. rewrite ! List.map_map in *.
+    rewrite List.app_assoc in *.
+    apply NoDup_app_disjoint with (a:=fn) in wf_fnsems0; ss.
+    + replace fn with (fst (fn, i)); et.
+      replace (List.map (fun x : string * (Any.t -> itree Es Any.t) => fst (trans_r (trans_l x)))) with (List.map (fun x : string * (Any.t -> itree Es Any.t) => fst x)).
+      2: { f_equal. extensionality x. rewrite fst_trans_r. rewrite fst_trans_l. et. }
+      apply in_app_iff. right. 
+      apply in_map. apply alist_find_some in MS1. et.
+    + replace fn with (fst (fn, i0)); et.
+      replace (fun x : string * (Any.t -> itree Es Any.t) => fst (trans_r (trans_r x))) with (fun x : string * (Any.t -> itree Es Any.t) => fst x).
+      2: { extensionality x. rewrite fst_trans_r. rewrite fst_trans_r. et. }
+      apply in_map. apply alist_find_some in MS2. et.
+  - right. right. esplits; et; s; et.
+    unfold sim_fsem, "==>". i. eapply add_assoc_aux; et.
+    rewrite H0.
+    erewrite <- ! (@bisimulation_is_eq _ _ _ _ (@translate_cmpE _ _ _ _ _ _ _)).
+    econs. econs.
+  - right. right. esplits; et; s; et.
+    unfold sim_fsem, "==>". i. eapply add_assoc_aux; et.
+    rewrite H0.
+    erewrite <- ! (@bisimulation_is_eq _ _ _ _ (@translate_cmpE _ _ _ _ _ _ _)).
+    econs. econs.
+  - s. et.
+Qed.
+
+Theorem add_assoc_rev
+        ms0 ms1 ms2
+        (P0 P1: Prop) (IMPL: P1 -> P0)
+        (WF: wf (add (add ms0 ms1) ms2))
+  :
+    <<COMM: Beh.of_program (compile (add ms0 (add ms1 ms2)) (Some P0)) <1=
+            Beh.of_program (compile (add (add ms0 ms1) ms2) (Some P1))>>
+.
+Proof.
+  destruct (classic (P1)); cycle 1.
+  { ii. eapply initial_itr_not_wf;et. }
+  replace P0 with P1.
+  2: { eapply prop_ext. split; auto. }
+  unfold compile. red. 
+  eapply adequacy_local_aux; et.
+  2: { exists tt. instantiate (1:= top2). instantiate (1:=(fun _ => assoc_rev_st)).  econs; et; clarify. 
+       unfold assoc_rev_st. ss. exists (init_st ms0), (init_st ms1), (init_st ms2). splits; et. }
+  i. s.
+  unfold add_fnsems, trans_l, trans_r. s. unfold add_fnsems, trans_l, trans_r. 
+  rewrite ! alist_find_app_o. rewrite ! alist_find_map. 
+  rewrite ! alist_find_app_o. rewrite ! alist_find_map. 
+
+  destruct (alist_find fn (fnsems ms0)) eqn: MS0; 
+  destruct (alist_find fn (fnsems ms1)) eqn:MS1; 
+  destruct (alist_find fn (fnsems ms2)) eqn: MS2;
+  ( ss; et; right; right; esplits; et; s; et; unfold sim_fsem, "==>"; i; eapply add_assoc_rev_aux; et; rewrite H0;
+    erewrite <- ! (@bisimulation_is_eq _ _ _ _ (@translate_cmpE _ _ _ _ _ _ _)); econs; econs).
+Qed.
+
+End ASSOC.
+
+Section EMPTY.
+
+Inductive empty_emb : IFun Es Es -> Prop := 
+  | empty_emb_intro : empty_emb emb_l
+.
+
+Inductive empty_ems : itree Es Any.t -> itree Es Any.t -> Prop := 
+  | empty_ems_intro emb_l it (EMB: empty_emb emb_l) :
+      empty_ems it (translate emb_l it).    
+
+Definition empty_st (stp: Any.t * Any.t) : Prop :=
+  exists a, fst stp = a /\ 
+  snd stp = Any.pair a tt↑
+.
+
+Lemma add_empty_aux
+        itl itr stl str (w: unit)
+        (EMPTY: empty_ems itl itr)
+        (STATE: empty_st (stl, str))
+
+  :
+      sim_itree (fun _ => empty_st) top2 false false w (stl, itl) (str, itr)
+.
+Proof.
+  destruct EMPTY, STATE. des. ss.
+  unfold empty_st.
+  ginit. 
+  generalize it as itr. 
+  clarify.
+  generalize x as a.
+  gcofix CIH. i.
+  rewrite (itree_eta_ itr).
+  destruct (observe itr).
+  - (* Ret *)
+    erewrite ! (bisimulation_is_eq _ _ (translate_ret _ _)).
+    gstep. apply sim_itree_ret.
+    unfold lift_rel. 
+    exists tt. splits; et.
+  - (* Tau *)
+    erewrite ! (bisimulation_is_eq _ _ (translate_tau _ _)).
+    gstep. 
+    apply sim_itree_tau_src. apply sim_itree_tau_tgt. 
+    eapply sim_itree_progress; et.
+    gfinal. left. eapply CIH; et.
+  - (* Vis *)
+    erewrite ! (bisimulation_is_eq _ _ (translate_vis _ _ _ _)).
+    rewrite <- ! bind_trigger.
+    destruct e as [c|[s|e]].
+    + (* callE *)
+      gstep. destruct c, EMB. 
+      apply sim_itree_call; clarify.
+      -- exists a; et.
+      -- i. destruct WF, H. ss. clarify.
+         gfinal. left. eapply CIH.
+    + (* sE *)
+      gstep. destruct s, EMB.
+      apply sim_itree_supdate_src. apply sim_itree_supdate_tgt.
+      eapply sim_itree_progress; et.
+      unfold run_l, run_r. rewrite ! Any.pair_split.
+      gfinal. left. destruct (run a). eapply CIH.
+      
+    + (* eventE *)
+      gstep. destruct e, EMB.
+      (* Choose *)
+      * apply sim_itree_choose_tgt. i. apply sim_itree_choose_src. exists x0.
+        eapply sim_itree_progress; et.
+        gfinal. left. eapply CIH.
+      (* Take *)
+        * apply sim_itree_take_src. i. apply sim_itree_take_tgt. exists x0.
+        eapply sim_itree_progress; et.
+        gfinal. left. eapply CIH. 
+      (* Syscall *)
+        * apply sim_itree_syscall. i.
+        eapply sim_itree_flag_down.
+        gfinal. left. eapply CIH. 
+
+Qed.
+
+Context {CONF: EMSConfig}.
+
+Theorem add_empty
+      ms
+      (P0 P1: Prop) (IMPL: P1 -> P0)
+      (WF: wf ms)
+:
+  <<EMPTY: Beh.of_program (compile (add ms empty) (Some P0)) <1=
+          Beh.of_program (compile ms (Some P1))>>
+.
+Proof. 
+  destruct (classic (P1)); cycle 1.
+  { ii. eapply initial_itr_not_wf;et. }
+  replace P0 with P1.
+  2: { eapply prop_ext. split; auto. }
+  unfold compile. red. 
+  eapply adequacy_local_aux; et.
+  2: { exists tt. instantiate (1:= top2). instantiate (1:= (fun _ => empty_st)). econs; et; clarify.
+       unfold empty_st. ss. exists (init_st ms). et. }
+  i. s.
+  unfold add_fnsems, trans_l, trans_r. s.
+  rewrite ! alist_find_app_o. rewrite ! alist_find_map. 
+  destruct (alist_find fn (fnsems ms)) eqn: MS; cycle 1.
+  - left. et.
+  - ss. right. right. esplits; et.
+    unfold sim_fsem, "==>". i. apply add_empty_aux; et.
+    rewrite H0. econs. econs.
+Qed.
+End EMPTY.
+
+End ModSemFacts.
+
+Module ModFacts.
+Import Mod.
+Section BEH.
+
+Context `{Sk.ld}.
+Context {CONF: EMSConfig}.
+
+
+Theorem add_comm
+        md0 md1
+  :
+    <<COMM: Beh.of_program (compile (add md0 md1)) <1= Beh.of_program (compile (add md1 md0))>>
+.
+
+Proof.
+ii. unfold compile in *.
+destruct (classic (ModSem.wf (enclose (add md1 md0)) /\ Sk.wf (sk (add md1 md0)))).
+2: { eapply ModSem.initial_itr_not_wf. ss. }
+ss. des. assert (SK: Sk.wf (Sk.add (sk md0) (sk md1))).
+{ apply Sk.wf_comm. auto. }
+rewrite Sk.add_comm; et.
+eapply ModSemFacts.add_comm; [| |et].
+{ i. split; auto. unfold enclose. ss. rewrite Sk.add_comm; et.
+  inv H2. inv H3. econs; ss.
+  unfold ModSem.add_fnsems in *.
+  rewrite ! List.map_app in *.
+  rewrite ! List.map_map in *.
+  replace (fun x : string * (Any.t -> itree Es Any.t) => fst (ModSem.trans_l x)) with (fun x : string * (Any.t -> itree Es Any.t) => fst x) in *.
+  2: { extensionality x. rewrite ModSemFacts.fst_trans_l. et. }
+  replace (fun x : string * (Any.t -> itree Es Any.t) => fst (ModSem.trans_r x)) with (fun x : string * (Any.t -> itree Es Any.t) => fst x) in *.
+  2: { extensionality x. rewrite ModSemFacts.fst_trans_r. et. }
+  eapply nodup_comm. et.
+}
+{ rewrite Sk.add_comm; et. }
+Qed.
+
+
+(* Lemma add_assoc' ms0 ms1 ms2:
+  add ms0 (add ms1 ms2) = add (add ms0 ms1) ms2.
+Proof.
+  unfold add. f_equal.
+  { extensionality skenv_link. ss. apply ModSem.add_assoc'. }
+  { ss. rewrite Sk.add_assoc. auto. }
+Qed. *)
+
+Theorem add_assoc
+        md0 md1 md2
+  :
+    <<ASSOC: Beh.of_program (compile (add md0 (add md1 md2))) <1=
+            Beh.of_program (compile (add (add md0 md1) md2))>>
+.
+Proof. 
+ii. unfold compile in *.
+destruct (classic (ModSem.wf (enclose (add (add md0 md1) md2)) /\ Sk.wf (sk (add (add md0 md1) md2)))).
+2: { eapply ModSem.initial_itr_not_wf. ss. }
+ss. des. assert (SK: Sk.wf (Sk.add (sk md0) (Sk.add (sk md1) (sk md2)))).
+{ rewrite Sk.add_assoc. apply H1. }
+
+Search Sk.t.
+
+(* Sk associativity required *)
+
+{ admit. }
+Admitted.
+(* 
+rewrite Sk.sort_add_assoc; et.
+eapply ModSemFacts.add_comm; [| |et].
+{ i. split; auto. unfold enclose. ss. rewrite Sk.sort_add_comm; et.
+  inv H1. inv H2. econs; ss.
+  unfold ModSem.add_fnsems in *.
+  rewrite ! List.map_app in *.
+  rewrite ! List.map_map in *.
+  replace (fun x : string * (Any.t -> itree Es Any.t) => fst (ModSem.trans_l x)) with (fun x : string * (Any.t -> itree Es Any.t) => fst x) in *.
+  2: { extensionality x. rewrite ModSemFacts.fst_trans_l. et. }
+  replace (fun x : string * (Any.t -> itree Es Any.t) => fst (ModSem.trans_r x)) with (fun x : string * (Any.t -> itree Es Any.t) => fst x) in *.
+  2: { extensionality x. rewrite ModSemFacts.fst_trans_r. et. }
+  eapply nodup_comm. et.
+}
+{ rewrite Sk.sort_add_comm; et. }
+
+ *)
+
+(* Qed. *)
+
+Theorem add_assoc_rev
+        md0 md1 md2
+  :
+    <<COMM: Beh.of_program (compile (add (add md0 md1) md2)) <1=
+            Beh.of_program (compile (add md0 (add md1 md2)))>>
+.
+Proof. Admitted.
+  (* rewrite add_assoc'. ss.
+Qed. *)
+
+Lemma add_empty_r 
+      md
+  : 
+    << EMPTY: Beh.of_program (compile (add md empty)) <1=
+              Beh.of_program (compile md)>>
+.
+Proof.
+ii. unfold compile in *.
+destruct (classic (ModSem.wf (enclose md) /\ Sk.wf (sk md))).
+2: { eapply ModSem.initial_itr_not_wf. ss. }
+ss. des. assert (SK: Sk.wf (Sk.add (sk md) Sk.unit)).
+{ rewrite Sk.add_unit_r. et.  }
+eapply ModSemFacts.add_empty; [|et|].
+- instantiate (1:= wf (add md empty)). i.
+  unfold wf. esplits; et. ss.
+  inv H0. econs. 
+  rewrite Sk.add_unit_r.
+  unfold ModSem.add, ModSem.add_fnsems. ss.
+  rewrite List.map_app. rewrite List.map_map.
+  ss. rewrite app_nil_r.
+  replace (fun x : string * (Any.t -> itree Es Any.t) => fst (ModSem.trans_l x)) with ((fun x : string * (Any.t -> itree Es Any.t) => fst x)).
+  2: { extensionality x. rewrite ModSemFacts.fst_trans_l. et. }
+  ss.
+  
+- unfold ModSem.compile, ModSem.empty, enclose.
+  rewrite Sk.add_unit_r in PR. et.
+  
+Qed.
+
+Lemma add_empty_l 
+      md
+  : 
+    << EMPTY: Beh.of_program (compile (add empty md)) <1=
+              Beh.of_program (compile md)>>
+.
+Proof. 
+(* empty_r + comm *)
+Admitted.
+
+
+(* Do we still add by list? (and refines2, refines_proper, etc.)
+Definition add_list (xs: list t): t :=
+  fold_right add empty xs
+.
+
+(* Lemma add_list_single: forall (x: t), add_list [x] = x.
+Proof. ii; cbn. rewrite add_empty_r. refl. Qed. *)
+
+Definition add_list_cons
+          x xs
+        :
+          (add_list (x::xs) = (add x (add_list xs)))
+.
+Proof. ss. Qed.
+
+Definition add_list_snoc
+          x xs
+        :
+          << SNOC: Beh.of_program (compile (add_list (snoc xs x))) <1= 
+                   Beh.of_program (compile (add (add_list xs) x)) >>
+.
+Proof. Admitted. *)
+
+  (* ginduction xs; ii; ss.
+  { cbn. rewrite add_empty_l, add_empty_r. et. }
+  { cbn. rewrite <- add_assoc'.  r in IHxs. r. f_equal.}  *)
+
+End BEH.
+End ModFacts.
+
+Section REFINE.
+  Context `{Sk.ld}.
+
+  Section CONF.
+  Context {CONF: EMSConfig}.
+
+  
+  (*** vertical composition ***)
+  Global Program Instance refines_PreOrder: PreOrder refines.
+
+  Next Obligation. ii. ss. Qed.
+  Next Obligation. ii. eapply H1. eapply H0. ss. Qed.
+
+
+  Global Program Instance refines_strong_PreOrder: PreOrder refines_strong.
+  Next Obligation. ii. ss. Qed.
+  Next Obligation. ii. eapply H1. eapply H0. ss. Qed.
+
+  Global Program Instance refines_closed_PreOrder: PreOrder refines_closed.
+  Next Obligation. ii; ss. Qed.
+  Next Obligation. ii; ss. eapply H1. eapply H0. eauto. Qed.
+
+  (*** horizontal composition ***)
+  Theorem refines_add
+        (md0_src md0_tgt md1_src md1_tgt: Mod.t)
+        (SIM0: refines md0_tgt md0_src)
+        (SIM1: refines md1_tgt md1_src)
+    :
+        <<SIM: refines (Mod.add md0_tgt md1_tgt) (Mod.add md0_src md1_src)>>
+  .
+  Proof. 
+    ii. r in SIM0. r in SIM1. 
+    pose proof ModFacts.add_comm as COMM. 
+    pose proof ModFacts.add_assoc as ASSOC. 
+    pose proof ModFacts.add_assoc_rev as ASSOC'. 
+    r in COMM. r in ASSOC. r in ASSOC'.
+    apply ASSOC'. 
+    apply SIM1.
+    apply ASSOC. apply COMM. apply ASSOC. apply COMM.
+    apply SIM0.
+    apply ASSOC. apply COMM. apply ASSOC.
+    apply PR.
+  Qed.
+
+  Lemma refines_close: refines <2= refines_closed.
+  Proof. 
+    ii. specialize (PR Mod.empty). ss.
+    pose proof ModFacts.add_empty_l as EMP.
+    r in EMP.
+    apply EMP with (x0 := x2) in PR.
+    2: { admit. (* empty_rev required. *) } 
+    apply PR.
+  Admitted.
+
+  End CONF.
+
+   Theorem refines_strong_add
+         (md0_src md0_tgt md1_src md1_tgt: Mod.t)
+         (SIM0: refines_strong md0_tgt md0_src)
+         (SIM1: refines_strong md1_tgt md1_src)
+     :
+       <<SIM: refines_strong (Mod.add md0_tgt md1_tgt) (Mod.add md0_src md1_src)>>
+   .
+   Proof.
+     intros CONF. eapply (@refines_add CONF); et.
+   Qed.
+   Lemma refines_strong_refines {CONF: EMSConfig}: refines_strong <2= refines.
+   Proof. ii. eapply PR; et. Qed.
+
+End REFINE.
+
