ems/SImModSemFacts.v
@@ -1,0 +1,333 @@
+Require Import Coqlib.
+Require Import ITreelib.
+Require Import Skeleton.
+Require Import ModSem.
+Require Import Behavior.
+Require Import Relation_Definitions.
+
+(*** TODO: export these in Coqlib or Universe ***)
+Require Import Relation_Operators.
+Require Import RelationPairs.
+From ITree Require Import
+     Events.MapDefault.
+From ExtLib Require Import
+     Core.RelDec
+     Structures.Maps
+     Data.Map.FMapAList.
+Require Import Any.
+
+Require Import SimGlobal.
+Require Import Red IRed.
+Require Import SimModSem.
+Require Import ModSemFacts.
+Import TAC.
+
+Section ADEQUACY.
+
+  Definition embl_st (stp: Any.t * Any.t) : Prop :=
+    exists a b c, (fst stp = Any.pair a b /\ 
+    snd stp = Any.pair a c).
+
+  Lemma sim_emb_l 
+    x x' (wf: unit -> Any.t * Any.t -> Prop) wf' (w:unit) it
+    (WF: wf tt (x, x'))
+    (WF': wf' = (fun _ '(stl, str) => match (Any.split stl), (Any.split str) with
+                                      | Some (xl, _), Some (xr, _) => wf tt (xl, xr)
+                                      | _, _ => False
+                                      end
+    ) )
+    (* (SIM: sim_itree wf top2 false false w (x, it) (x', it)) *)
+    (SIM: sim_fsem wf top2 (fun _ => it) (fun _ => it))
+  :
+    forall x1 x2, sim_itree wf' top2 false false w (Any.pair x x1, translate ModSem.emb_l it)
+    (Any.pair x' x2, translate ModSem.emb_l it)
+  .
+  Proof.
+    ginit. 
+    generalize it as itr.
+    revert WF. 
+    generalize x as a.
+    generalize x' as b.
+    gcofix CIH. i.
+    rewrite (itree_eta_ itr).
+    destruct (observe itr).
+    - (* Ret *)
+    erewrite ! (bisimulation_is_eq _ _ (translate_ret _ _)).
+    gstep. apply sim_itree_ret.
+    unfold lift_rel. 
+    exists w. splits; et. rewrite WF'. rewrite ! Any.pair_split. et.
+  - (* Tau *)
+    erewrite ! (bisimulation_is_eq _ _ (translate_tau _ _)).
+    gstep. 
+    apply sim_itree_tau_src. apply sim_itree_tau_tgt. 
+    eapply sim_itree_progress; et.
+    gfinal. left. eapply CIH; et.
+  - (* Vis *)
+    erewrite ! (bisimulation_is_eq _ _ (translate_vis _ _ _ _)).
+    rewrite <- ! bind_trigger.
+    destruct e as [c|[s|e']].
+    + (* callE *)
+      gstep. destruct c.
+      eapply sim_itree_call; clarify.
+      -- rewrite ! Any.pair_split. apply WF.
+      -- i. des_ifs. 
+         gfinal. left. apply Any.split_pair in Heq. apply Any.split_pair in Heq0.
+         des. clarify. eapply CIH. apply WF0.
+    + (* sE *)
+      gstep. destruct s.
+      apply sim_itree_supdate_src. apply sim_itree_supdate_tgt.
+      eapply sim_itree_progress; et.
+      unfold ModSem.run_l. rewrite ! Any.pair_split.
+      gfinal. left. destruct (run a), (run b). ss. eapply CIH.
+      
+    + (* eventE *)
+      gstep. destruct e, EMB.
+      (* Choose *)
+      * apply sim_itree_choose_tgt. i. apply sim_itree_choose_src. exists x0.
+        eapply sim_itree_progress; et.
+        gfinal. left. eapply CIH.
+      (* Take *)
+        * apply sim_itree_take_src. i. apply sim_itree_take_tgt. exists x0.
+        eapply sim_itree_progress; et.
+        gfinal. left. eapply CIH. 
+      (* Syscall *)
+        * apply sim_itree_syscall. i.
+        eapply sim_itree_flag_down.
+        gfinal. left. eapply CIH. 
+  Admitted.
+
+  Theorem adequacy_local_strong md_src md_tgt
+          (SIM: ModPair.sim md_src md_tgt)
+    :
+    <<CR: (refines_strong md_tgt md_src)>>
+  .
+  Proof. 
+  (* Admitted. *)
+    ii. 
+    unfold Mod.compile, Mod.enclose in *.
+    destruct (classic (Mod.wf (Mod.add ctx md_src))).
+    2:{ eapply ModSem.compile_not_wf. ss. }
+    pose (sk_tgt := (Mod.sk (Mod.add ctx md_tgt))).
+    pose (sk_src := (Mod.sk (Mod.add ctx md_src))).
+    assert (SKEQ: sk_tgt = sk_src).
+    { unfold sk_src, sk_tgt. ss. f_equal.
+      inv SIM. auto. }
+    rr in H.
+    unfold Mod.enclose in *. fold sk_src in H. des. inv WF.
+    rename SK into SKWF.
+    rename wf_fnsems into FNWF.
+    inv SIM. hexploit (sim_modsem (Sk.canon sk_tgt)).
+    { etrans; [|eapply Sk.sort_incl]. ss. ii. eapply in_or_app. auto. }
+    { ss. 
+      fold sk_src in SKWF. 
+      rewrite SKEQ. 
+      clear - SKWF.
+      unfold Sk.wf in *. ss. eapply Permutation.Permutation_NoDup; [|et].
+      eapply Permutation.Permutation_map. eapply Sk.SkSort.sort_permutation. }
+    i. inv H. des.
+    assert (WFTGT: Mod.wf (Mod.add ctx md_tgt)).
+    { rr. unfold Mod.enclose. fold sk_src sk_tgt. 
+      rewrite SKEQ in *. split; auto. econs.
+      match goal with
+        | H: NoDup ?l0 |- NoDup ?l1 => replace l1 with l0
+      end; auto. ss. unfold ModSem.add_fnsems.
+      rewrite ! List.map_app. f_equal. rewrite ! List.map_map.
+      eapply Forall2_eq. eapply Forall2_apply_Forall2; et.
+      i. destruct a, b. inv H. ss.
+    }
+
+    eapply adequacy_local_aux in PR; et.
+
+    { ss. ii. fold sk_src sk_tgt. rewrite <- SKEQ.
+      unfold ModSem.add_fnsems. rewrite ! alist_find_app_o. des_ifs.
+      { eapply alist_find_some in Heq.
+        eapply in_map_iff in Heq. des. destruct x. ss. clarify.
+        right. left.
+        exists i0, (Mod.get_modsem ctx (Sk.sort sk_tgt)), (Mod.get_modsem md_src (Sk.sort sk_tgt)), (Mod.get_modsem md_tgt (Sk.sort sk_tgt)).
+        esplits; et.
+        - apply alist_find_some_iff; et.
+          unfold ModSem.add_fnsems in FNWF. rewrite List.map_app in FNWF.
+          apply nodup_app_l in FNWF. rewrite List.map_map in FNWF.
+          revert FNWF.
+          replace (fun x : string * (Any.t -> itree Es Any.t) => fst (ModSem.trans_l x)) with (fun x : string * (Any.t -> itree Es Any.t) => fst x).
+          2: { extensionality x. rewrite ModSemFacts.fst_trans_l. refl. }
+          rewrite SKEQ. i. et.
+        - unfold sim_fsem, "==>". i. clarify.
+          instantiate (1:= top2). instantiate (1:= unit). instantiate (1:= (fun _ => embl_st)). 
+          ss. unfold embl_st in SIMMRS. ss. inv SIMMRS. inv H. inv H0. inv H.
+          eapply sim_emb_l. destruct w. eapply self_sim_itree.
+          unfold ModSem.emb_l, ModSem.run_l. ss.
+          
+          2: { et.  }
+        
+        et. des. inv sim_fnsems0.
+        destruct b. esplits; ss; et. erewrite alist_find_some_iff; et.
+
+
+        admit.
+
+      }
+      {
+        
+      }
+
+
+      destruct (ModSem.fnsems (Mod.get_modsem CTX (Sk.sort sk_tgt)) fn) eqn:Hctx.
+      - right. admit.
+      -  
+      (* revert_until SKEQ. *)
+      (* pattern (Sk.sort sk_tgt) at 1. *)
+      (* rewrite <- SKEQ. rewrite ! alist_find_app_o. des_ifs. *)
+
+      esplits. instantiate (1:= le).
+      instantiate (1:= wf_lift wf).
+      unfold sim_fnsem in *.
+      (* revert fn. *)
+
+      hexploit (sim_fnsems fn). i.
+      
+      revert_until SKEQ.
+      generalize (Mod.get_modsem md_src (Sk.sort sk_tgt)) as ms_src. 
+      generalize (Mod.get_modsem md_tgt (Sk.sort sk_tgt)) as ms_tgt.
+      unfold ModSemAdd.add_fnsems.
+      i. des_ifs; et; right.
+      - exists (fun _ : Any.t => triggerUB), (fun _ : Any.t => triggerUB). 
+        esplits; et. 
+        unfold sim_fsem, "==>". i.
+        ginit. gstep. econs. ss.
+      - exists (fun args : Any.t => translate ModSemAdd.emb_l (i args)), (fun args : Any.t => translate ModSemAdd.emb_l (i args)).
+        esplits; et.
+        unfold sim_fsem, "==>". i. rewrite H1.
+        unfold wf_lift in SIMMRS. des_ifs.
+        +  
+        ginit. gstep. econs.
+
+      generalize (ModSemAdd.add_fnsems (Mod.get_modsem ctx (Sk.sort sk_tgt)) ms_src) as o_src. 
+      generalize (ModSemAdd.add_fnsems (Mod.get_modsem ctx (Sk.sort sk_tgt)) ms_tgt) as o_tgt.
+      i.
+      destruct o_src, o_tgt; et; right.
+      - exists i, i0. esplits; et. apply sim_fnsems. 
+      destruct (ModSem.fnsems ms_src fn); cycle 1.
+      - left. et.
+      - right. exists i.
+    
+      
+      
+      exists i. destruct o_tgt; cycle 1. 
+        + eexists. splits; et. instantiate (1:= le). instantiate (1:=wf).
+          splits.
+          *     
+        + exists i0. splits; et.
+          unfold sim_fsem, respectful'. ii.
+
+      (* - right. destruct (ModSem.add_fnsems (Mod.get_modsem ctx (Sk.sort sk_tgt))
+        (Mod.get_modsem md_tgt (Sk.sort sk_tgt)) fn).
+        + exists i. exists i0. splits; et.
+          unfold sim_fsem, respectful'. i. inv H0.
+     *)
+    
+    rewrite <- SKEQ. rewrite ! alist_find_app_o. des_ifs.
+      { eapply alist_find_some in Heq.
+        rewrite Mod.add_list_fnsems in Heq.
+        rewrite <- fold_right_app_flat_map in Heq. ss.
+        eapply in_flat_map in Heq. des.
+        eapply in_map_iff in Heq0. des. destruct x1. ss. clarify.
+        right. left. esplits; ss; et.
+        instantiate (1:=ModSem.mn (Mod.get_modsem md_src (Sk.sort sk_tgt))).
+        ii. eapply NoDup_app_disjoint.
+        { rewrite List.map_app in MNWF. eapply MNWF. }
+        { rewrite Mod.add_list_initial_mrs.
+          rewrite <- fold_right_app_flat_map. eapply in_map.
+          eapply in_flat_map. ss. esplits; et. }
+        { ss. rewrite <- SKEQ. rewrite H. auto. }
+      }
+      { rewrite ! alist_find_map_snd. uo. des_ifs_safe ltac:(auto).
+        eapply alist_find_some in Heq0. right. right.
+        eapply Forall2_In_l in sim_fnsems; et. des. inv sim_fnsems0.
+        destruct b. esplits; ss; et. erewrite alist_find_some_iff; et.
+        { rewrite sim_mn. ss; et. }
+        { inv WFTGT. inv H1. ss. rewrite List.map_app in wf_fnsems.
+          apply nodup_app_r in wf_fnsems.
+          rewrite List.map_map in wf_fnsems. ss. fold sk_tgt in wf_fnsems.
+          erewrite List.map_ext; et. i. destruct a. ss.
+        }
+        { ss. inv H. ss. clarify. }
+      }
+    }
+    { exists w_init. econs.
+      { refl. }
+      { ss. 
+        instantiate (1:=wf).
+        
+        unfold ModSem.initial_p_state.
+        erewrite ! alist_find_some_iff; et.
+        { clear FNWF.
+          match goal with
+          | H: NoDup ?l0 |- NoDup ?l1 => replace l1 with l0
+          end; auto. ss.
+          fold sk_src. fold sk_tgt. rewrite <- SKEQ.
+          rewrite ! List.map_app. f_equal. ss. f_equal. auto.
+        }
+        { ss. eapply in_or_app. right. ss. left. fold sk_tgt. f_equal. auto. }
+        { ss. eapply in_or_app. right. ss. left. fold sk_src. rewrite SKEQ. auto. }
+      }
+      { ii. ss. fold sk_src sk_tgt. rewrite SKEQ. unfold ModSem.initial_p_state.
+        ss. rewrite ! alist_find_app_o. des_ifs_safe.
+        rewrite <- SKEQ. ss. rewrite ! eq_rel_dec_correct. des_ifs. }
+    }
+  Qed.
+
+  Context {CONF: EMSConfig}.
+
+  Theorem adequacy_local md_src md_tgt
+          (SIM: ModPair.sim md_src md_tgt)
+    :
+      <<CR: (refines md_tgt md_src)>>
+  .
+  Proof.
+    eapply refines_strong_refines.
+    eapply adequacy_local_strong; et.
+  Qed.
+
+  (* Corollary adequacy_local_list_strong
+            mds_src mds_tgt
+            (FORALL: List.Forall2 ModPair.sim mds_src mds_tgt)
+    :
+      <<CR: refines_strong (Mod.add_list mds_tgt) (Mod.add_list mds_src)>>
+  .
+  Proof. Admitted. *)
+
+
+    (* r. induction FORALL; ss.
+    { ii. auto. }
+    (* rewrite ! Mod.add_list_cons. *)
+    etrans.
+    { rewrite <- Mod.add_list_single. eapply refines_strong_proper_r.
+      rewrite ! Mod.add_list_single. eapply adequacy_local_strong; et. }
+    replace (Mod.lift x) with (Mod.add_list [x]); cycle 1.
+    { cbn. rewrite Mod.add_empty_r. refl. }
+    eapply refines_strong_proper_l; et.
+  Qed. *)
+
+  (* Theorem adequacy_local2 md_src md_tgt
+          (SIM: ModPair.sim md_src md_tgt)
+    :
+      <<CR: (refines2 [md_tgt] [md_src])>>
+  .
+  Proof.
+    eapply ModSem.refines_strong_refines.
+    eapply adequacy_local_list_strong. econs; ss.
+  Qed. *)
+
+  (* Corollary adequacy_local_list
+            mds_src mds_tgt
+            (FORALL: List.Forall2 ModPair.sim mds_src mds_tgt)
+    :
+      <<CR: refines (Mod.add_list mds_tgt) (Mod.add_list mds_src)>>
+  .
+  Proof.
+    eapply ModSem.refines_strong_refines.
+    eapply adequacy_local_list_strong; et.
+  Qed. *)
+
+End ADEQUACY.
