ems/SimGlobal.v
@@ -509,7 +509,7 @@ Qed.
 
 
 Lemma step_trigger_choose_iff X k itr e
-      (STEP: ModSemL.step (trigger (Choose X) >>= k) e itr)
+      (STEP: ModSem.step (trigger (Choose X) >>= k) e itr)
   :
     exists x,
       e = None /\ itr = k x.
@@ -524,7 +524,7 @@ Proof.
 Qed.
 
 Lemma step_trigger_take_iff X k itr e
-      (STEP: ModSemL.step (trigger (Take X) >>= k) e itr)
+      (STEP: ModSem.step (trigger (Take X) >>= k) e itr)
   :
     exists x,
       e = None /\ itr = k x.
@@ -539,7 +539,7 @@ Proof.
 Qed.
 
 Lemma step_tau_iff itr0 itr1 e
-      (STEP: ModSemL.step (Tau itr0) e itr1)
+      (STEP: ModSem.step (Tau itr0) e itr1)
   :
     e = None /\ itr0 = itr1.
 Proof.
@@ -547,7 +547,7 @@ Proof.
 Qed.
 
 Lemma step_ret_iff rv itr e
-      (STEP: ModSemL.step (Ret rv) e itr)
+      (STEP: ModSem.step (Ret rv) e itr)
   :
     False.
 Proof.
@@ -555,7 +555,7 @@ Proof.
 Qed.
 
 Lemma step_trigger_syscall_iff fn args rvs k e itr
-      (STEP: ModSemL.step (trigger (Syscall fn args rvs) >>= k) e itr)
+      (STEP: ModSem.step (trigger (Syscall fn args rvs) >>= k) e itr)
   :
     exists rv, itr = k rv /\ e = Some (event_sys fn args rv)
                /\ <<RV: rvs rv>> /\ <<SYS: syscall_sem (event_sys fn args rv)>>.
@@ -582,11 +582,11 @@ Qed.
 
 Lemma step_trigger_choose X k x
   :
-    ModSemL.step (trigger (Choose X) >>= k) None (k x).
+    ModSem.step (trigger (Choose X) >>= k) None (k x).
 Proof.
   unfold trigger. ss.
   match goal with
-  | [ |- ModSemL.step ?itr _ _] =>
+  | [ |- ModSem.step ?itr _ _] =>
     replace itr with (Subevent.vis (Choose X) k)
   end; ss.
   { econs. }
@@ -596,11 +596,11 @@ Qed.
 
 Lemma step_trigger_take X k x
   :
-    ModSemL.step (trigger (Take X) >>= k) None (k x).
+    ModSem.step (trigger (Take X) >>= k) None (k x).
 Proof.
   unfold trigger. ss.
   match goal with
-  | [ |- ModSemL.step ?itr _ _] =>
+  | [ |- ModSem.step ?itr _ _] =>
     replace itr with (Subevent.vis (Take X) k)
   end; ss.
   { econs. }
@@ -611,11 +611,11 @@ Qed.
 Lemma step_trigger_syscall fn args (rvs: Any.t -> Prop) k rv
       (RV: rvs rv) (SYS: syscall_sem (event_sys fn args rv))
   :
-    ModSemL.step (trigger (Syscall fn args rvs) >>= k) (Some (event_sys fn args rv)) (k rv).
+    ModSem.step (trigger (Syscall fn args rvs) >>= k) (Some (event_sys fn args rv)) (k rv).
 Proof.
   unfold trigger. ss.
   match goal with
-  | [ |- ModSemL.step ?itr _ _] =>
+  | [ |- ModSem.step ?itr _ _] =>
     replace itr with (Subevent.vis (Syscall fn args rvs) k)
   end; ss.
   { econs; et. }
@@ -625,7 +625,7 @@ Qed.
 
 Lemma step_tau itr
   :
-    ModSemL.step (Tau itr) None itr.
+    ModSem.step (Tau itr) None itr.
 Proof.
   econs.
 Qed.
@@ -636,9 +636,9 @@ Hypothesis (FINSAME: (@finalize CONFS) = (@finalize CONFT)).
 Theorem adequacy_global_itree itr_src itr_tgt
         (SIM: simg eq false false itr_src itr_tgt)
   :
-    Beh.of_program (@ModSemL.compile_itree CONFT itr_tgt)
+    Beh.of_program (@ModSem.compile_itree CONFT itr_tgt)
     <1=
-    Beh.of_program (@ModSemL.compile_itree CONFS itr_src).
+    Beh.of_program (@ModSem.compile_itree CONFS itr_src).
 Proof.
   unfold Beh.of_program. ss.
   remember false as o_src0 in SIM at 1.
@@ -686,15 +686,16 @@ Proof.
 Qed.
 
 
-Variable md_src md_tgt: ModL.t.
-Let ms_src: ModSemL.t := md_src.(ModL.enclose).
-Let ms_tgt: ModSemL.t := md_tgt.(ModL.enclose).
+Variable md_src md_tgt: Mod.t.
+Let ms_src: ModSem.t := md_src.(Mod.enclose).
+Let ms_tgt: ModSem.t := md_tgt.(Mod.enclose).
 
 Section ADEQUACY.
-Hypothesis (SIM: simg eq false false (@ModSemL.initial_itr ms_src CONFS (Some (ModL.wf md_src))) (@ModSemL.initial_itr ms_tgt CONFT (Some (ModL.wf md_tgt)))).
+(* Hypothesis (SIM: simg eq false false (@ModSem.initial_itr ms_src CONFS ) (@ModSem.initial_itr ms_tgt CONFT )). *)
+Hypothesis (SIM: simg eq false false (@ModSem.initial_itr ms_src CONFS (Some (Mod.wf md_src))) (@ModSem.initial_itr ms_tgt CONFT (Some (Mod.wf md_tgt)))).
 
 
-Theorem adequacy_global: Beh.of_program (@ModL.compile _ CONFT md_tgt) <1= Beh.of_program (@ModL.compile _ CONFS md_src).
+Theorem adequacy_global: Beh.of_program (@Mod.compile _ CONFT md_tgt) <1= Beh.of_program (@Mod.compile _ CONFS md_src).
 Proof.
   eapply adequacy_global_itree. eapply SIM.
 Qed.
@@ -765,3 +766,38 @@ Proof.
   { econs; eauto. }
   { econs; eauto. }
 Qed.
+
+(* Lemma simg_map R0 R1 RR R0' R1' RR' f_src f_tgt itl itr (f0: R0 -> R0') (f1: R1 -> R1')
+      (SIM: @simg R0 R1 RR f_src f_tgt itl itr)
+      (IMPL: forall r0 r1, RR r0 r1 -> RR' (f0 r0) (f1 r1): Prop)
+:
+      @simg R0' R1' RR' f_src f_tgt (f0 <$> itl) (f1 <$> itr)
+.
+Proof.
+  revert_until RR'.
+  pcofix CIH. i.
+  (* punfold SIM.  *)
+  induction SIM using simg_ind; s.
+  - erewrite ! (bisimulation_is_eq _ _ (map_ret _ _)). eauto with paco.
+  - erewrite ! (bisimulation_is_eq _ _ (map_bind _ _ _)).
+    pfold. apply simg_syscall. i. right. eapply CIH; et.
+    (* specialize (SIM _ _ EQ). pclearbot. et. *)
+    (* edestruct SIM; et. inv H. *)
+  - erewrite ! (bisimulation_is_eq _ _ (map_tau _ _)).
+    pfold. apply simg_tauL; et. punfold IHSIM.
+  - erewrite ! (bisimulation_is_eq _ _ (map_tau _ _)). 
+    pfold. apply simg_tauR; et. punfold IHSIM.
+  - erewrite ! (bisimulation_is_eq _ _ (map_bind _ _ _)).
+    pfold. apply simg_chooseL; et. 
+    des. exists x. punfold IH.
+  - erewrite ! (bisimulation_is_eq _ _ (map_bind _ _ _)).
+    pfold. apply simg_chooseR; et.
+    i. exploit SIM. esplits. des. punfold IH.
+  - erewrite ! (bisimulation_is_eq _ _ (map_bind _ _ _)).
+    pfold. apply simg_takeL; et.
+    i. exploit SIM. esplits. des. punfold IH.
+  - erewrite ! (bisimulation_is_eq _ _ (map_bind _ _ _)).
+    pfold. apply simg_takeR; et.
+    des. exists x. punfold IH.
+  - pfold. apply simg_progress; et. right. eapply CIH; et.
+Qed. *)
